Finished the proof that the closure conversion algorithm is in the closure conversion relation (in the file closure_conversion_corresp.v). General cleanup will follow.

certicoq/theories/L6_PCPS/closure_conversion_correct.v
@@ -81,7 +81,7 @@ Lemma Fun_inv_set k rho rho' Scope Funs σ Γ f rho1 B1 f1 rho2 B2 f2 tau t vs:
   Fun_inv k rho rho' Scope Funs σ Γ ->
   (σ f) <> Γ ->
   ~ In _ Scope (σ f) ->
-  ~ In _ (image σ Funs) (σ f) ->
+  ~ In _ (image σ (Setminus _ Funs Scope)) (σ f) ->
   M.get Γ rho' = Some (Vconstr tau t vs) ->
   (exists tau' t',
      cc_approx_val k (Vfun rho1 B1 f1)
@@ -103,12 +103,12 @@ Proof.
     + inv Hin; eauto. inv H. congruence.
     + subst. repeat eexists; eauto. rewrite M.gso. now eauto. 
       intros Hc. inv Hin. inv H. congruence. eapply Hinj. 
-      rewrite <- Hc. eexists; eauto.
+      rewrite <- Hc. eexists; split; [| now eauto]. now constructor; eauto.
 Qed.
 
 (** Rename the environment parameter *)
 Lemma Fun_inv_rename k rho1 rho2 Scope Funs σ Γ Γ' v :
-  ~ In _ (image σ Funs) Γ ->  ~ In _ (image σ Funs) Γ' ->
+  ~ In _ (image σ (Setminus _ Funs Scope)) Γ ->  ~ In _ (image σ Funs) Γ' ->
   Fun_inv k rho1 (M.set Γ v rho2) Scope Funs σ Γ ->
   Fun_inv k rho1 (M.set Γ' v rho2) Scope Funs σ Γ'.
 Proof.
@@ -120,7 +120,8 @@ Proof.
       [rhof1 [B1 [f1 [rhof2 [B2 [f2 [tau' [t' [Heq [Hnin'' [Hget' Happrox']]]]]]]]]]]; eauto.
   rewrite M.gsspec in Hget'.
   destruct (Coqlib.peq (σ f) Γ); subst.
-  - exfalso. eapply Hnin. eexists. eauto.
+  - exfalso. eapply Hnin. eexists. split; [| now eauto ].
+    constructor; eauto.
   - destruct (Coqlib.peq (σ f) Γ'); subst.
     + exfalso. eapply Hnin'. eexists. eauto.
     + repeat eexists; eauto. rewrite M.gso; eauto.
@@ -128,7 +129,7 @@ Qed.
 
 (** Extend [Scope] with a set that does not shadow the new function names *)
 Lemma Fun_inv_mon k rho1 rho2 Scope Scope' Funs σ Γ :
-  Disjoint _ (image σ Funs) Scope' ->
+  Disjoint _ (image σ (Setminus _ Funs Scope)) Scope' ->
   Fun_inv k rho1 rho2 Scope Funs σ Γ ->
   Fun_inv k rho1 rho2 (Union _ Scope' Scope) Funs σ Γ.
 Proof.
@@ -139,7 +140,7 @@ Proof.
       [rhof1 [B1 [f1 [rhof2 [B2 [f2 [tau' [t' [Heq [Hnin'' [Hget'' Happrox']]]]]]]]]]]; eauto.
   repeat eexists; eauto.
   intros Hc; inv Hc; eauto. eapply Hd. constructor; eauto.
-  eexists; eauto.
+  eexists; eauto. split; [| now eauto ]. constructor; eauto.
 Qed.
 
 (** Extend the first environment with a variable in [Scope] *)
@@ -158,7 +159,7 @@ Qed.
 
 (** Extend the second environment with a variable in [Scope] *)
 Lemma Fun_inv_set_In_Scope_r k rho1 rho2 Scope Funs σ Γ x v v' :
-  In _ Scope x ->  ~ In _ (image σ Funs) x ->
+  In _ Scope x ->  ~ In _ (image σ (Setminus _ Funs Scope)) x ->
   Fun_inv k rho1 (M.set Γ v rho2) Scope Funs σ Γ ->
   Fun_inv k rho1 (M.set Γ v (M.set x v' rho2)) Scope Funs σ Γ.
 Proof.
@@ -174,6 +175,7 @@ Proof.
   - repeat eexists; try eassumption.
     rewrite M.gso; eauto. rewrite M.gso. eassumption. 
     intros Heq''; subst. eapply Hnin. eexists; eauto.
+    split; [| now eauto]. constructor; eauto.
 Qed.
 
 (** Extend the second environment with a variable in [Scope] that is different
@@ -197,7 +199,7 @@ Qed.
 (** Extend the second environment with a variable not in [Funs] that is different
     from Γ *)
 Lemma Fun_inv_set_not_In_Funs_r_not_Γ k rho1 rho2 Scope Funs σ Γ x v :
-   ~ In _ (image σ Funs) x ->
+   ~ In _ (image σ (Setminus _ Funs Scope)) x ->
    x <> Γ -> 
    Fun_inv k rho1 rho2 Scope Funs σ Γ ->
    Fun_inv k rho1 (M.set x v rho2) Scope Funs σ Γ.
@@ -238,7 +240,8 @@ Qed.
 
 (** Extend the second environment with a list of variables in [Scope] *)
 Lemma Fun_inv_setlist_In_Scope_r k rho1 rho2 rho2' Scope Funs σ Γ xs vs v :
-  Included _ (FromList xs) Scope -> Disjoint _ (image σ Funs) (FromList xs) ->
+  Included _ (FromList xs) Scope ->
+  Disjoint _ (image σ (Setminus _ Funs Scope)) (FromList xs) ->
   Fun_inv k rho1 (M.set Γ v rho2) Scope Funs σ Γ ->
   setlist xs vs rho2 = Some rho2' ->
   Fun_inv k rho1 (M.set Γ v rho2') Scope Funs σ Γ.
@@ -310,7 +313,7 @@ Qed.
 (** Define a block of functions in the first environment and put the in the
     current scope *)
 Lemma Fun_inv_def_funs_l k rho rho' B1 B1' Scope Funs σ Γ:
-  Disjoint _ (image σ Funs) (name_in_fundefs B1') -> 
+  Disjoint _ (image σ (Setminus _ Funs Scope)) (name_in_fundefs B1') -> 
   Fun_inv k rho rho' Scope Funs σ Γ ->
   Fun_inv k (def_funs B1 B1' rho rho) rho'
           (Union _ (name_in_fundefs B1')  Scope) Funs σ Γ.
@@ -323,14 +326,15 @@ Proof.
       [rhof1 [B1'' [f1 [rhof2 [B2 [f2 [tau' [t' [Heq [Hnin' [Hget'' Hcc]]]]]]]]]]];
     eauto.
    repeat eexists; eauto. intros Hc; inv Hc; eauto.
-   eapply Hd. econstructor; eauto. now eexists; eauto.
+   eapply Hd. econstructor; eauto.
+   eexists; split; [| now eauto ]. constructor; eauto.
 Qed.
 
 (** Define a block of functions in the second environment and put the in the
     current scope *)
 Lemma Fun_inv_def_funs_r k rho rho' B1 B1' Scope Funs σ Γ:
   ~ In _ (name_in_fundefs B1') Γ ->
-  Disjoint _ (image σ Funs) (name_in_fundefs B1') -> 
+  Disjoint _ (image σ (Setminus _ Funs Scope)) (name_in_fundefs B1') -> 
   Fun_inv k rho rho' Scope Funs σ Γ ->
   Fun_inv k rho (def_funs B1 B1' rho' rho')
           (Union _ (name_in_fundefs B1') Scope) Funs σ Γ.
@@ -343,17 +347,19 @@ Proof.
       [rho1' [B2 [f1 [rho2' [B2' [f2 [tau2 [t2 [Heq' [Hnin' [Hget2 Happrox2]]]]]]]]]]]; eauto.
   repeat eexists; eauto.
   intros Hc; inv Hc; eauto.
-  eapply Hd. econstructor; eauto. now eexists; eauto.
+  eapply Hd. econstructor; eauto. eexists;  split; [| now eauto ].
+  now constructor; eauto.
   rewrite def_funs_neq; eauto.
-  intros Hc. eapply Hd. constructor; eauto. now eexists; eauto.
+  intros Hc. eapply Hd. constructor; eauto. eexists; split; [| now eauto ].
+  now constructor; eauto.
 Qed.
 
 (** Define a block of functions in both environments and put the in the
     current scope *)
 Lemma Fun_inv_def_funs k rho rho' B1 B1' B2 B2' Scope Funs σ Γ:
   ~ In _ (name_in_fundefs B2') Γ -> ~ In _ (name_in_fundefs B1') Γ ->
-  Disjoint _ (image σ Funs) (name_in_fundefs B1') ->
-  Disjoint _ (image σ Funs) (name_in_fundefs B2') ->
+  Disjoint _ (image σ (Setminus _ Funs Scope)) (name_in_fundefs B1') ->
+  Disjoint _ (image σ (Setminus _ Funs Scope)) (name_in_fundefs B2') ->
   (* Same_set _ (name_in_fundefs B1') (name_in_fundefs B2') -> *)
   Fun_inv k rho rho' Scope Funs σ Γ ->
   Fun_inv k  (def_funs B1 B1' rho rho) (def_funs B2 B2' rho' rho')
@@ -369,9 +375,11 @@ Proof.
       [rho1' [B3 [f1 [rho2' [B3' [f2 [tau2 [t2 [Heq' [Hnin2 [Hget2 Happrox2]]]]]]]]]]]; eauto.
   repeat eexists; eauto.
   intros Hc; inv Hc; eauto.
-  eapply Hd. econstructor; eauto. now eexists; eauto.
+  eapply Hd. econstructor; eauto. eexists; split; [| now eauto ].
+  now constructor; eauto.
   rewrite def_funs_neq; eauto.
-  intros Hc. eapply Hd'. econstructor; eauto. now eexists; eauto.
+  intros Hc. eapply Hd'. econstructor; eauto. eexists; split; [| now eauto ].
+  now constructor; eauto.
 Qed.
 
 (** * Lemmas about FV_inv *)
@@ -648,13 +656,16 @@ Proof.
   intros Hinj Hcc Hdef. induction Hcc.
   - simpl in Hdef. destruct (M.elt_eq f f0) eqn:Heq; subst.
     + inv Hdef. repeat eexists; eauto.
+      simpl.
+      intros Hc. eapply H. now eauto.
       simpl. rewrite Coqlib.peq_true. reflexivity.
     + edestruct IHHcc as [t2 [Γ'' [C' [e2 [Hnin [Hfind Hcc']]]]]]; eauto.
       eapply injectiveP_antimon. eassumption.
       now apply Included_Union_r.
       repeat eexists; eauto. simpl. rewrite Coqlib.peq_false. eassumption.
       intros Hc. eapply n. eapply Hinj; eauto.
-      right. eapply fun_in_fundefs_name_in_fundefs. eapply find_def_correct. now eauto.
+      right. eapply fun_in_fundefs_name_in_fundefs.
+      eapply find_def_correct. now eauto.
       left; eauto.
   - inv Hdef.
 Qed.
@@ -689,24 +700,37 @@ Proof.
   intros Hin x [y [Hin' Heq]]; subst. eexists; eauto.
 Qed.
 
-Lemma make_closures_image_Included B S σ Γ C S' σ' :
-  make_closures B S σ Γ C S' σ' ->
-  Included _ (image σ' (name_in_fundefs B)) S.
+Instance image_Proper_Same_set {A B} : Proper (eq ==> Same_set A ==> Same_set B) image.
+Proof.
+  intros x1 x2 Heq1 s1 s2 Hseq; subst; split; intros x [y [Hin Heq]]; subst;
+  eexists; split; eauto; apply Hseq; eauto.
+Qed.
+
+Instance image_Proper_f_eq {A B} : Proper (f_eq ==> eq ==> Same_set B) (@image A B).
+Proof.
+  intros x1 x2 Heq1 s1 s2 Hseq; subst; split; intros x [y [Hin Heq]]; subst;
+  eexists; split; eauto; apply Hseq; eauto.
+Qed.
+
+Lemma make_closures_image_Included B S Γ C σ S' :
+  make_closures B S Γ C σ S' ->
+  Included _ (image σ (name_in_fundefs B)) S.
 Proof. 
   intros Hmc. induction Hmc.
   - rewrite image_Empty_set. apply Included_Empty_set.
-  - simpl.
+  - simpl. subst. 
     rewrite image_Union, image_Singleton.
     apply Union_Included. apply Singleton_Included.
-    now rewrite extend_gss.
-    eapply Included_trans. now apply image_extend_Included.
+    rewrite <- H0. rewrite extend_gss. eassumption.
+    eapply Included_trans.
+    rewrite <- H0. now apply image_extend_Included.
     apply Union_Included.
     eapply Included_trans. eassumption. now eapply Subset_Setminus.
     now apply Singleton_Included.
 Qed.
 
-Lemma make_closures_free_set_Included B S σ Γ C S' σ' :
-  make_closures B S σ Γ C S' σ' ->
+Lemma make_closures_free_set_Included B S Γ C σ S' :
+  make_closures B S Γ C σ S' ->
   Included _  S' S.
 Proof. 
   intros Hmc. induction Hmc.
@@ -742,31 +766,39 @@ Proof.
       inv Hin2. inv H; congruence. eassumption.
 Qed.
 
-Lemma make_closures_image_Disjoint B S σ Γ C S' σ' :
-  make_closures B S σ Γ C S' σ' ->
-  Disjoint _ (image σ' (name_in_fundefs B)) S'.
-Proof. 
+Lemma make_closures_image_Disjoint B S Γ C σ S' :
+  make_closures B S Γ C σ S' ->
+  Disjoint _ (image σ (name_in_fundefs B)) S'.
+Proof.
   intros Hmc. induction Hmc.
   - rewrite image_Empty_set. apply Disjoint_Empty_set_l.
   - simpl. rewrite image_Union, image_Singleton.
-    rewrite extend_gss. eapply Disjoint_Union.
+    rewrite <- H0. rewrite extend_gss. eapply Disjoint_Union.
     + eapply Disjoint_Included_r.
       now eapply make_closures_free_set_Included; eauto.
-      apply Disjoint_sym. apply Disjoint_Setminus. now apply Included_refl. 
-    + eapply Disjoint_Included_l. now apply image_extend_Included.
+      apply Disjoint_sym. apply Disjoint_Setminus. now apply Included_refl.
+    + eapply Disjoint_Included_l. rewrite <- H0.
+      now apply image_extend_Included.
       apply Disjoint_Union. eassumption.
       eapply Disjoint_Included_r. now eapply make_closures_free_set_Included; eauto.
       apply Disjoint_sym. eapply Disjoint_Setminus. now apply Included_refl.
 Qed.
 
-Lemma make_closures_injective B S σ Γ C S' σ' :
+Instance injectiveP_Proper {A B} : Proper (f_eq ==> eq ==> iff) (@injectiveP A B).
+Proof.
+  intros f1 f2 Hfeq s1 s2 Hseq; split; intros Hinj x y Hin1 Hin2 Heq; subst;
+  eapply Hinj; eauto. now rewrite !Hfeq. now rewrite <- !Hfeq. 
+Qed.
+
+Lemma make_closures_injective B S Γ C σ S' :
   Disjoint _ S (name_in_fundefs B) ->
-  make_closures B S σ Γ C S' σ' ->
-  injectiveP σ' (name_in_fundefs B).
+  make_closures B S Γ C  σ S' ->
+  injectiveP σ (name_in_fundefs B).
 Proof. 
   intros Hd Hmc. induction Hmc.
   - intros x y Hc. inv Hc. 
-  - simpl. eapply injectiveP_extend. 
+  - simpl. rewrite <- H0.
+    eapply injectiveP_extend.
     + eapply IHHmc.
       eapply Disjoint_Included_r; [| eapply Disjoint_Included_l; [| eassumption ] ].
       now apply Included_Union_r.
@@ -803,7 +835,7 @@ Qed.
 Lemma project_var_not_In_free_set  Scope Funs σ Γ FVs x x' C S S'  :
   project_var Scope Funs σ Γ FVs S x x' C S' ->
   Disjoint _ S (Union var Scope
-                      (Union var (image σ Funs)
+                      (Union var (image σ (Setminus _ Funs Scope))
                              (Union var (FromList FVs) (Singleton var Γ)))) ->
   ~ In _ S' x'.
 Proof.
@@ -816,7 +848,7 @@ Qed.
 Lemma project_vars_not_In_free_set Scope Funs σ Γ FVs xs xs' C S S'  :
   project_vars Scope Funs σ Γ FVs S xs xs' C S' ->
   Disjoint _ S (Union var Scope
-                      (Union var (image σ Funs)
+                      (Union var (image σ (Setminus _ Funs Scope))
                              (Union var (FromList FVs) (Singleton var Γ)))) ->
   Disjoint _ S' (FromList xs').
 Proof.
@@ -1001,15 +1033,15 @@ Proof.
     eexists. econstructor; eauto. constructor. 
 Qed.
 
-Lemma make_closures_ctx_to_rho B S σ Γ C S' σ' k rho1 rho2 :
-  make_closures B S σ Γ C S' σ' ->
+Lemma make_closures_ctx_to_rho B S Γ C σ S' k rho1 rho2 :
+  make_closures B S Γ C σ S' ->
   unique_functions B ->
   Disjoint _ S (name_in_fundefs B) ->
   ~ In _ (name_in_fundefs B) Γ ->
-  Fun_inv k rho1 rho2 (Empty_set _) (name_in_fundefs B) σ' Γ ->
+  Fun_inv k rho1 rho2 (Empty_set _) (name_in_fundefs B) σ Γ ->
   (forall f, In _ (name_in_fundefs B) f -> exists v, M.get f rho1 = Some v) ->
   exists rho2', ctx_to_rho C rho2 rho2'.
-Proof. 
+Proof.
   intros Hclo. revert rho1 rho2. induction Hclo; intros rho1 rho2 Hun Hd Hnin Hfun Hyp. 
   - eexists; constructor. 
   - destruct (Hyp f) as [v' Hget'].
@@ -1025,25 +1057,27 @@ Proof.
       now apply Included_Union_r.
     + intros Hc; eapply Hnin; right; eauto.
     + eapply Fun_inv_set_not_In_Funs_r_not_Γ with (x := f).
+      rewrite Setminus_Empty_set_Same_set.
       intros Hin. eapply make_closures_image_Included in Hclo.
-      eapply Hd. constructor; [| now left; eauto ].
-      eapply Hclo. eassumption. 
+      eapply Hd.  constructor; [| now left; eauto ].
+      eapply Hclo. eassumption.
       intros Hc; subst. eapply Hnin. now left; eauto.
-      do 3 eexists; split; eauto; intros.
+      do 3 eexists. split; eauto. intros. 
       edestruct Hfun' as
           [rho1'' [B1' [f1' [rho2'' [B2' [f2' [tau2' [t2' [Heq'' [Hnin'' [Hget2' Happrox2']]]]]]]]]]]; eauto.
       right; eauto.
       subst. repeat eexists; eauto. intros Hc; inv Hc.
-      unfold extend in Hget2'. rewrite Coqlib.peq_false in Hget2'. eassumption.
+      rewrite <- H0 in Hget2'. unfold extend in Hget2'.
+      rewrite Coqlib.peq_false in Hget2'. eassumption.
       intros Hc; subst; contradiction.
     + intros. eapply Hyp. right; eauto.
-    + eexists. econstructor; eauto.
+    + eexists. econstructor; eauto. rewrite <- H0 in Hget2. 
       unfold extend in Hget2. rewrite Coqlib.peq_true in Hget2. eassumption.
 Qed.
 
 Lemma project_vars_ctx_to_rho Scope Funs σ Γ FVs xs xs' C S S' vs1 k rho1 rho2 :
   Disjoint _ S (Union var Scope
-                      (Union var (image σ Funs)
+                      (Union var (image σ (Setminus _ Funs Scope))
                              (Union var (FromList FVs) (Singleton var Γ)))) ->
   project_vars Scope Funs σ Γ FVs S xs xs' C S' ->
   Fun_inv k rho1 rho2 Scope Funs σ Γ ->
@@ -1053,7 +1087,6 @@ Lemma project_vars_ctx_to_rho Scope Funs σ Γ FVs xs xs' C S S' vs1 k rho1 rho2
 Proof. 
   intros HD Hvars Hfun [tau [t [vs [Hget Henv]]]].
   assert (HD' := Hvars).
-  (* apply project_vars_Disjoint in HD'; [ | eassumption ].  *)
   revert Scope Funs Γ FVs xs' C S S' vs1 tau t vs k
          rho1 rho2  HD HD' Hvars Hfun Hget Henv. 
   induction xs;
@@ -1128,7 +1161,7 @@ Lemma Closure_conversion_fundefs_correct k rho rho' B1 B2 B1' B2'
         binding_in_map (occurs_free e) rho ->
         fundefs_names_unique e ->
         injectiveP σ Funs ->
-        Disjoint var (image σ Funs) (bound_var e) ->
+        Disjoint var (image σ (Setminus _ Funs Scope)) (bound_var e) ->
         Fun_inv m rho rho' Scope Funs σ Γ ->
         FV_inv m rho rho' Scope Funs Γ FVs ->
         Closure_conversion Scope Funs σ Γ FVs e e' C ->
@@ -1164,7 +1197,7 @@ Proof.
       * intros B H. inv H; eauto. specialize (Hun' (Fcons v t l e B1') (or_intror eq_refl)).
         inv Hun'; eauto.
       * eapply Disjoint_Included_l; [| eassumption ].
-        eapply image_monotonic. now apply Included_Union_r.
+        eapply image_monotonic.  now apply Included_Union_r.
       * eapply injectiveP_antimon. eassumption. now apply Included_Union_r.
       * intros Hc. apply Hnin1'. simpl; eauto.
       * intros Hc. apply Hnin2'. simpl; eauto.
@@ -1173,6 +1206,7 @@ Proof.
       left. eauto.
     + simpl in Hinj'. eapply injectiveP_Union_Disjoint in Hinj'.
       intros Hc. eapply Hinj'. constructor; eauto. eexists; eauto.
+      eapply image_monotonic; [| eassumption ]. now apply Subset_Setminus.
       eapply Disjoint_sym. eapply Disjoint_Singleton.
       specialize (Hun' (Fcons v t l e B1') (or_intror eq_refl)).
       inv Hun'; eauto.
@@ -1207,7 +1241,9 @@ Proof.
         eapply fun_in_fundefs_funs_in_fundef; eauto.
         eapply find_def_correct. eassumption.
       * now eapply Hinj.
-      * eapply Disjoint_Included_r; [| now apply Hd ].
+      * eapply Disjoint_Included_r;
+        [| eapply Disjoint_Included_l;
+           [ apply image_monotonic; now apply Subset_Setminus | now apply Hd ] ].
         eapply Included_trans;
           [| eapply fun_in_fundefs_bound_var_fundefs; now eapply find_def_correct; eauto ].
         rewrite !Union_assoc. now apply Included_Union_r.
@@ -1227,11 +1263,15 @@ Proof.
             eexists; split; eauto. eapply cc_approx_val_monotonic.
             eassumption. omega. } 
         eapply Fun_inv_rename with (Γ := Γ).
-        intros Hin. eapply Hseq in Hin. contradiction.
+        intros Hin.
+        eapply Hnin2. rewrite <- Hseq. eapply image_monotonic; [| eassumption ].
+        now apply Subset_Setminus.
         intros Hin. eapply Hnin''. left; eassumption.
         eapply Fun_inv_setlist_In_Scope_l; [ now apply Included_refl | |].
         eapply Fun_inv_setlist_In_Scope_r; [ now apply Included_refl | | | eassumption ].  
-        eapply Disjoint_Included_r; [|  eassumption ].
+        eapply Disjoint_Included_r;
+          [| eapply Disjoint_Included_l;
+             [ apply image_monotonic; now apply Subset_Setminus | now apply Hd ]].
         eapply Included_trans;
           [| eapply fun_in_fundefs_bound_var_fundefs; now eapply find_def_correct; eauto ].
         right; eauto.
@@ -1262,7 +1302,7 @@ Lemma project_var_correct k rho1 rho2 rho2'
   FV_inv k rho1 rho2 Scope Funs Γ FVs ->
   ctx_to_rho C rho2 rho2' ->
   Disjoint _ S (Union var Scope
-                      (Union var (image σ Funs)
+                      (Union var (image σ (Setminus _ Funs Scope))
                              (Union var (FromList FVs) (Singleton var Γ)))) ->
   ~ In _ S' x' /\
   cc_approx_env_P Scope k rho1 rho2' /\
@@ -1288,7 +1328,7 @@ Proof.
       subst. repeat eexists; eauto.
       rewrite M.gso. eassumption. 
       intros Hc. subst; eapply Hd; constructor; eauto. right; left.
-      eexists; eauto.
+      eexists. split; [| now eauto ]. constructor; eauto.
     + eapply FV_inv_set_r. now intros Heq; subst; eapply Hd; eauto.
       eassumption.
     + intros v Hget. eexists. rewrite M.gss. split; eauto.
@@ -1312,7 +1352,7 @@ Proof.
       subst. repeat eexists; eauto.
       rewrite M.gso. eassumption. 
       intros Hc. subst; eapply Hd; eauto. constructor; eauto. right; left.
-      eexists; eauto.
+      eexists. split; [| now eauto ]. constructor; eauto.      
     + eapply FV_inv_set_r. now intros Heq; subst; eapply Hd; eauto.
       eassumption.
     + intros v' Hget. eexists. rewrite M.gss. split; eauto.
@@ -1331,7 +1371,7 @@ Lemma project_vars_correct k rho1 rho2 rho2'
   FV_inv k rho1 rho2 Scope Funs Γ FVs ->
   ctx_to_rho C rho2 rho2' ->
   Disjoint _ S (Union var Scope
-                      (Union var (image σ Funs)
+                      (Union var (image σ (Setminus _ Funs Scope))
                              (Union var (FromList FVs) (Singleton var Γ)))) ->
   cc_approx_env_P Scope k rho1 rho2' /\
   Fun_inv k rho1 rho2' Scope Funs σ Γ /\
@@ -1364,23 +1404,21 @@ Proof.
     erewrite <- project_vars_get; eauto. rewrite Hget'''. reflexivity.
 Qed.
 
-
-
 (** Correctness of [make_closures] *)
-Lemma make_closures_correct k rho1 rho2 rho2' B S σ Γ' C S' σ' σ'' Scope Funs FVs Γ :
-  make_closures B S σ Γ' C S' σ' ->
+Lemma make_closures_correct k rho1 rho2 rho2' B S Γ' C σ S' σ' Scope Funs FVs Γ :
+  make_closures B S Γ' C σ S' ->
   unique_functions B ->
   ~ In _ (name_in_fundefs B) Γ ->
   ~ In _ (name_in_fundefs B) Γ' ->
   Included _ (name_in_fundefs B) Scope ->
   Disjoint _ S (name_in_fundefs B) ->
   cc_approx_env_P (Setminus _ Scope (name_in_fundefs B)) k rho1 rho2 ->
-  Fun_inv k rho1 rho2 Scope Funs σ'' Γ ->  
+  Fun_inv k rho1 rho2 Scope Funs σ' Γ ->  
   FV_inv k rho1 rho2 Scope Funs Γ FVs ->
-  Fun_inv k rho1 rho2 (Empty_set _) (name_in_fundefs B) σ' Γ' ->
+  Fun_inv k rho1 rho2 (Empty_set _) (name_in_fundefs B) σ Γ' ->
   ctx_to_rho C rho2 rho2' ->
   cc_approx_env_P Scope k rho1 rho2' /\
-  Fun_inv k rho1 rho2' Scope Funs σ'' Γ /\
+  Fun_inv k rho1 rho2' Scope Funs σ' Γ /\
   FV_inv k rho1 rho2' Scope Funs Γ FVs.
 Proof.
   intros Hmake. revert k rho1 rho2 rho2' Scope Funs FVs Γ.
@@ -1392,7 +1430,7 @@ Proof.
     now rewrite Setminus_Empty_set_Same_set in Hcc. 
   - eapply ctx_to_rho_comp_ctx_l in Hctx; [| apply Constr_cc; constructor ].
     destruct Hctx as [rho2'' [Hctx1 Hctx2]].
-    inv Hctx1. inv H10. inv Hun.
+    inv Hctx1. inv H11. inv Hun.
     edestruct IHHmake as [Hcc1 [Hfun1 Henv1]];
       [ eassumption | | | | | | | | | eassumption | ].  
     + intros Hc. eapply Hnin1. right. now apply Hc. 
@@ -1413,10 +1451,10 @@ Proof.
       edestruct Hfun2
         as [rho1f' [B1 [f1 [rho2f' [B2 [f2 [tau2' [t2' [Heq' [Hnin2' [Hget2' Happrox2]]]]]]]]]]];
       [| | eassumption |]. now eapply not_In_Empty_set. now left; eauto.
-      unfold extend in Hget2'. rewrite Coqlib.peq_true in Hget2'. 
-      subst. eexists; split. 
+      rewrite <- H0 in Hget2'. unfold extend in Hget2'. rewrite Coqlib.peq_true in Hget2'.
+      subst. eexists; split.
       rewrite M.gss. reflexivity.
-      rewrite H8 in Hget2. inv Hget2. rewrite H9 in Hget2'. inv Hget2'.
+      rewrite H9 in Hget2. inv Hget2. rewrite H10 in Hget2'. inv Hget2'.
       rewrite cc_approx_val_eq in *. simpl. now eauto.
     + eapply Fun_inv_set_In_Scope_r_not_Γ ; [| | eassumption ].
       * eapply Hsub. now left. 
@@ -1433,7 +1471,7 @@ Proof.
         [| | eassumption |].
       now eapply not_In_Empty_set. now right; eauto.
       repeat eexists; eauto. intros Hc; now inv Hc. 
-      rewrite M.gso. unfold extend in Hget2'.  
+      rewrite <- H0 in Hget2'. rewrite M.gso. unfold extend in Hget2'.  
       rewrite Coqlib.peq_false in Hget2'. eassumption.
       intros Hc; subst. contradiction.
       eapply make_closures_image_Included in Hmake. intros Hc; subst.
@@ -1465,7 +1503,7 @@ Lemma Closure_conversion_correct k rho rho' e e' Scope Funs σ Γ FVs C :
   (* function renaming is injective in the [Funs] subdomain *)
   injectiveP σ Funs ->
   (* function renaming codomain is not shadowed by other vars *)
-  Disjoint _ (image σ Funs) (bound_var e) ->
+  Disjoint _ (image σ (Setminus _ Funs Scope)) (bound_var e) ->
   (* [Fun] invariant *)
   Fun_inv k rho rho' Scope Funs σ Γ ->
   (* Free variables invariant *)
@@ -1498,8 +1536,11 @@ Proof.
     + eapply binding_in_map_antimon; [| eapply binding_in_map_set; eassumption ].
       eapply occurs_free_Econstr_Included. 
     + intros f Hfin. eauto.
-    + eapply Disjoint_Included_r; [| eassumption ].
+    + eapply Disjoint_Included_r;
+      [| eapply Disjoint_Included_l; [ apply image_monotonic | now apply Hd ]].
       rewrite bound_var_Econstr. now apply Included_Union_l.
+      apply Included_Setminus_compat.
+      now apply Included_refl. now apply Included_Union_r.
     + eapply Fun_inv_set_In_Scope_l. now eauto.
       eapply Fun_inv_set_In_Scope_r_not_Γ. now eauto.
       intros Heq; subst. now eauto.
@@ -1625,8 +1666,11 @@ Proof.
     + eapply binding_in_map_antimon; [| eapply binding_in_map_set; eassumption ].
       eapply occurs_free_Eproj_Included. 
     + intros f Hfin. eauto.
-    + eapply Disjoint_Included_r; [| eassumption ].
+    + eapply Disjoint_Included_r;
+      [| eapply Disjoint_Included_l; [ apply image_monotonic | now apply Hd ]].
       rewrite bound_var_Eproj. now apply Included_Union_l.
+      apply Included_Setminus_compat.
+      now apply Included_refl. now apply Included_Union_r.
     + eapply Fun_inv_set_In_Scope_l. now eauto.
       eapply Fun_inv_set_In_Scope_r_not_Γ. now eauto.
       intros Heq; subst. now eauto.
@@ -1647,7 +1691,7 @@ Proof.
     intros v1 c1 Hleq Hstep.
     edestruct project_vars_ctx_to_rho as [rho2' Hto_rho]; [ | eassumption | | | | ]; eauto.
     edestruct project_vars_correct as [Happ [Hfun' [Henv' Hvar]]]; eauto.
-    edestruct Hvar as [v' [Hget' Happ']]; eauto.
+    edestruct Hvar as [v' [Hget' Happ']]; eauto. rewrite <- app_ctx_f_fuse.
     eapply ctx_to_rho_cc_approx_exp; eauto.
     assert (Hsuf :
               cc_approx_exp k (e, def_funs f2 f2 rho1 rho1)
@@ -1789,8 +1833,11 @@ Proof.
             rewrite Union_sym. now apply Included_refl.
             apply binding_in_map_def_funs. eassumption.
           * intros f Hfin; eauto.
-          * eapply Disjoint_Included_r; [| eassumption ].
-            rewrite bound_var_Efun. now apply Included_Union_r. }
+          * eapply Disjoint_Included_r;
+            [| eapply Disjoint_Included_l; [ apply image_monotonic | now apply Hd ]].
+            rewrite bound_var_Efun. now apply Included_Union_r.
+            apply Included_Setminus_compat.
+            now apply Included_refl. now apply Included_Union_r. }
     intros v1' c1' Hleq' Hstep'. inv Hstep'.
     edestruct Hsuf as [v2' [c2' [Hstep2' Hcc2']]]; [| eassumption |]; eauto.
     repeat eexists; eauto. econstructor; eauto.
@@ -1870,8 +1917,11 @@ Proof.
     + eapply binding_in_map_antimon; [| eapply binding_in_map_set; eassumption ].
       eapply occurs_free_Eprim_Included. 
     + intros f Hfin. eauto.
-    + eapply Disjoint_Included_r; [| eassumption ].
+    + eapply Disjoint_Included_r;
+      [| eapply Disjoint_Included_l; [ apply image_monotonic | now apply Hd ]].
       rewrite bound_var_Eprim. now apply Included_Union_l.
+      apply Included_Setminus_compat.
+      now apply Included_refl. now apply Included_Union_r.
     + eapply Fun_inv_set_In_Scope_l. now eauto.
       eapply Fun_inv_set_In_Scope_r_not_Γ. now eauto.
       intros Heq; subst. now eauto.
@@ -1883,1324 +1933,3 @@ Proof.
     + repeat eexists; [| eassumption ].
       econstructor; eauto.
 Admitted.
-
-(** * Correspondance of the relational and the computational definitions of closure conversion *)
-
-Require Import hoare ExtLib.Structures.Monads ExtLib.Data.Monads.StateMonad alpha_conv List_util.
-
-Open Scope alpha_scope.
-
-Section CC_correct.
-  Context (utag : tag) (* Tag for types with unique constructor *)
-          (env_tag : tag) (* Tag for the type of environments *)
-          (tag_bij : tag -> tag) (* mapping from function tags to closure 
-                                    records tags *)
-          (unknown_type : type).
-
-
-  Open Scope ctx_scope.
-
-  (** All the variables greater or equal to x are in S (i.e. the "fresh" set) *)
-  Definition fresh (S : Ensemble var) (x : var) :=
-    forall y, (x <= y)%positive -> In _ S y.
-
-  (** Free variable map invariant *)
-  Definition FVmap_inv (FVmap : VarInfoMap) Scope Funs FVs : Prop :=
-    Same_set _ Scope (fun x => exists t, M.get x FVmap = Some (BoundVar t)) /\
-    Same_set _ (Setminus _ Funs Scope)
-             (fun x => exists x' t t', M.get x FVmap = Some (MRFun x' t t')) /\
-    forall N x, (nthN FVs N = Some x /\ ~ In _ Scope x /\ ~ In _ Funs x) <->
-           (exists t, M.get x FVmap = Some (FVar N t)).
-
-  (** Function names substitution *)
-  Definition subst (FVmap : VarInfoMap) x : var :=
-    match M.get x FVmap with
-      | Some (MRFun x' _ _) => x'
-      | _ => x
-    end.
-
-  Opaque bind ret.
-
-  (** A function that corresponds to an evaluation context *)
-  Definition is_exp_ctx (f : exp -> exp) C : Prop := 
-    forall e, f e = app_ctx_f C e. 
-
-  (** Set of variables not in the map *)
-  Definition binding_not_in_map {A} (S : Ensemble M.elt) (map : M.t A) := 
-    forall x : M.elt, In M.elt S x -> M.get x map = None.
-
-  (** Spec for [get_name] *)
-  Lemma get_name_fresh S :
-    {{ fun s => fresh S (fst s) }}
-      get_name
-    {{ fun _ x s' => fresh S x /\ fresh (Setminus var S (Singleton var x)) (fst s') }}.  
-  Proof.   
-    eapply pre_post_mp_l.
-    eapply bind_triple. eapply get_triple.
-    intros [x d] [x' d'].
-    eapply pre_post_mp_l. eapply bind_triple.
-    eapply put_triple. intros u [x'' d'']. eapply return_triple.
-    intros [x''' d'''] Heq1 [Heq2 Heq3] H. inv Heq1. inv Heq2. inv Heq3. 
-    split; eauto. intros y Hleq.
-    constructor.
-    - eapply H. simpl in *. zify. omega.
-    - intros Hin. inv Hin. simpl in *. eapply Pos.le_nlt in Hleq.
-      eapply Hleq. zify. omega.
-  Qed.
-  
-  Lemma fresh_monotonic S S' x :
-    Included _ S S' ->
-    fresh S x ->
-    fresh S' x.
-  Proof.
-    intros Hinc Hf x' Hleq. eapply Hinc. eapply Hf. eassumption.
-  Qed.
-
-  (** Spec for [get_var] *)
-  Lemma get_var_project_var_sound Scope Funs Γ FVs FVmap S x :
-    binding_in_map (Singleton _ x) FVmap ->
-    binding_not_in_map (Union _ S (Singleton _ Γ)) FVmap ->
-    FVmap_inv FVmap Scope Funs FVs ->
-    {{ fun s => fresh S (fst s) }}
-      get_var utag x FVmap Γ
-    {{ fun _ t s' =>
-         exists C S', 
-           fresh S' (fst s') /\
-           let '(x', _, f) := t in
-           (forall σ, f_eq σ (subst FVmap) ->
-                 project_var Scope Funs σ Γ FVs S x x' C S') /\
-           (subst FVmap) x' = x' /\
-           is_exp_ctx f C }}.
-  Proof.
-    intros Hin Hnin Minv. destruct Minv as [Minv1 [Minv2 Minv3]]. 
-    unfold get_var. edestruct (Hin x) as [inf Hget]; eauto. 
-    destruct inf; rewrite Hget. 
-    - eapply bind_triple.
-      + eapply get_name_fresh.     
-      + intros x' s. eapply return_triple. intros s' [Hf Hf'].
-        eexists (Eproj_c x' t n Γ Hole_c). repeat eexists. 
-        * eassumption.
-        * edestruct Minv3 as [H1 [H2 [H3 H4]]]. now repeat eexists; eauto.
-          econstructor 3; eauto.
-          eapply Hf. zify; omega.
-        * unfold subst. rewrite Hnin; eauto.
-          left. eapply Hf. zify; omega.
-    - eapply bind_triple.
-      + eapply get_name_fresh.  
-      + intros x' s. eapply return_triple. intros s' [Hf Hf'].
-        edestruct Minv2 as [H1 H2]; eauto. 
-        exists (Econstr_c x' t0 utag [v; Γ] Hole_c). repeat eexists.
-        * eassumption.
-        * intros σ Hfeq.
-          replace v with (σ x) by (rewrite Hfeq; unfold subst; rewrite Hget; reflexivity).
-          econstructor; eauto.
-          intros Hc. eapply Minv1 in Hc. destruct Hc as [t' Heq]. congruence.
-          eapply H2. repeat eexists; eauto.
-          eapply Hf. zify; omega.
-        * unfold subst. rewrite Hnin; eauto.
-          left. eapply Hf. zify; omega.
-    - eapply return_triple. intros [s d] Hin'.      
-      exists Hole_c. repeat eexists. 
-      + eassumption. 
-      + constructor. eapply Minv1. eexists; eauto.
-      + unfold subst. rewrite Hget; eauto.
-  Qed.
-
-  Lemma FVmap_inv_set_bound FVmap Scope Funs FVs x t :
-    FVmap_inv FVmap Scope Funs FVs ->
-    FVmap_inv (M.set x (BoundVar t) FVmap) (Union _ (Singleton _ x) Scope) Funs FVs.
-  Proof. 
-    intros [H1 [H2 H3]]. repeat split.
-    - intros y Hin. destruct (Coqlib.peq y x); subst.
-      + eexists. now rewrite M.gsspec, Coqlib.peq_true.
-      + inv Hin. inv H; congruence.
-        eapply H1 in H. edestruct H as [t' Heq].
-        eexists.  rewrite M.gsspec, Coqlib.peq_false; eauto.
-    - intros y Hin. destruct (Coqlib.peq y x); subst.
-      + eauto.
-      + edestruct Hin as [t' Heq]. rewrite M.gsspec, Coqlib.peq_false in Heq; [| now eauto ].
-        right. eapply H1. eexists; eauto.
-    - intros y Hin. inv Hin. destruct (Coqlib.peq y x); subst.
-      + exfalso. eauto.
-      + edestruct H2 as [H2' _].
-        edestruct H2' as [x' [t' [t'' Heq]]].
-        * constructor; eauto.
-        * eexists.  rewrite M.gsspec, Coqlib.peq_false; eauto.
-    - eapply H2. destruct H as [x' [t' [t'' Heq]]].
-      destruct (Coqlib.peq x x0); subst.
-      + rewrite M.gsspec, Coqlib.peq_true in Heq. congruence.
-      + repeat eexists. rewrite M.gsspec, Coqlib.peq_false in Heq; eauto.
-    - intros Hc. destruct H as [x' [t' [t'' Heq]]].
-      destruct (Coqlib.peq x0 x); subst.
-      + rewrite M.gsspec, Coqlib.peq_true in Heq. congruence.
-      + inv Hc. inv H; congruence.
-        eapply H2; eauto. repeat eexists.
-        rewrite M.gsspec, Coqlib.peq_false in Heq; eauto.
-    - intros [Hnth [Hnin Hnin']].
-      destruct (Coqlib.peq x0 x); subst.
-      + exfalso. eauto. 
-      + edestruct H3 as [[t' Heq] _].
-        now repeat split; eauto.
-        eexists. rewrite M.gsspec, Coqlib.peq_false; eauto.
-    - edestruct H as [t' Heq]. 
-      destruct (Coqlib.peq x0 x); subst.
-      + rewrite M.gsspec, Coqlib.peq_true in Heq. congruence.
-      + eapply H3; eauto.
-        rewrite M.gsspec, Coqlib.peq_false in Heq; eauto.
-    - edestruct H as [t' Heq]. 
-      destruct (Coqlib.peq x0 x); subst.
-      + rewrite M.gsspec, Coqlib.peq_true in Heq. congruence.
-      + intros Hc. inv Hc. inv H0; congruence.
-        rewrite M.gsspec, Coqlib.peq_false in Heq; eauto.
-        edestruct H3 as [_ [_ [Hc _]]].
-        eapply H3 in H0; eauto. contradiction.
-    - edestruct H as [t' Heq]. 
-      destruct (Coqlib.peq x0 x); subst.
-      + rewrite M.gsspec, Coqlib.peq_true in Heq. congruence.
-      + intros Hc.
-        rewrite M.gsspec, Coqlib.peq_false in Heq; eauto.
-        edestruct H3 as [_ [_ [_ Hc']]].
-        eapply H3 in Hc; eauto. contradiction.
-  Qed.
-
-  Lemma FVmap_inv_set_funs FVmap Scope Funs FVs x x' t t' :
-    ~ In _ Scope x ->
-    FVmap_inv FVmap Scope Funs FVs ->
-    FVmap_inv (M.set x (MRFun x' t t') FVmap) Scope (Union _ (Singleton _ x) Funs) FVs.
-  Proof. 
-    intros Hnin [H1 [H2 H3]]. repeat split.
-    - intros y Hin. destruct (Coqlib.peq y x); subst.
-      + contradiction.
-      + eapply H1 in Hin. edestruct Hin as [t'' Heq].
-        eexists.  rewrite M.gsspec, Coqlib.peq_false; eauto.
-    - intros y Hin. destruct (Coqlib.peq y x); subst.
-      + edestruct Hin as [t'' Heq]. rewrite M.gss in Heq; congruence.
-      + edestruct Hin as [t'' Heq]. rewrite M.gso in Heq; [| now eauto ].
-        eapply H1. eexists; eauto.
-    - intros y Hin. inv Hin. destruct (Coqlib.peq y x); subst.
-      + repeat eexists. rewrite M.gss. reflexivity.
-      + edestruct H2 as [H2' _].
-        edestruct H2' as [x'' [t'' [t''' Heq]]].
-        inv H. inv H4; congruence. constructor; eassumption.
-        repeat eexists. rewrite M.gso; eassumption.
-    - destruct (Coqlib.peq x0 x); subst; eauto. right.
-      eapply H2. edestruct H as [x'' [t1 [t2 Hget]]].
-      rewrite M.gso in Hget; [| now eauto ].
-      repeat eexists; eauto. 
-    - destruct H as [x'' [t1 [t2 Hget]]].
-      destruct (Coqlib.peq x0 x); subst; eauto.
-      rewrite M.gso in Hget; [| now eauto ].
-      intros Hc. apply H1 in Hc. edestruct Hc as [t3 Hget']. congruence.
-    - intros [Hnth [Hnin1 Hnin2]].
-      destruct (Coqlib.peq x0 x); subst.
-      + exfalso. eauto.
-      + edestruct H3 as [[t1 Heq] _].
-        now repeat split; eauto.
-        eexists. rewrite M.gsspec, Coqlib.peq_false; eauto.
-    - edestruct H as [t1 Heq].
-      destruct (Coqlib.peq x0 x); subst.
-      + rewrite M.gsspec, Coqlib.peq_true in Heq. congruence.
-      + eapply H3; eauto.
-        rewrite M.gsspec, Coqlib.peq_false in Heq; eauto.
-    - edestruct H as [t1 Heq].
-      destruct (Coqlib.peq x0 x); subst.
-      + rewrite M.gss in Heq. congruence.
-      + intros Hc.
-        rewrite M.gso in Heq; eauto. eapply H1 in Hc. 
-        edestruct Hc as [t2 Heq']. congruence.
-    - edestruct H as [t1 Heq].
-      destruct (Coqlib.peq x0 x); subst.
-      + rewrite M.gss in Heq. congruence.
-      + intros Hc.
-        rewrite M.gso in Heq; eauto.
-        inv Hc. inv H0; congruence.
-        edestruct H2 as [H2' _].  edestruct (H2' x0) as [y [t2 [t3 Hge']]].
-        constructor. eauto. intros Hc. eapply H1 in Hc. 
-        edestruct Hc as [t2 Heq']. congruence.
-        congruence.
-  Qed.
-
-  (** Spec for [get_vars] *)
-  Lemma get_vars_project_vars_sound Scope Funs Γ FVs FVmap S xs :
-    binding_in_map (FromList xs) FVmap ->
-    binding_not_in_map (Union _ S (Singleton _ Γ)) FVmap ->
-    FVmap_inv FVmap Scope Funs FVs ->
-    {{ fun s => fresh S (fst s) }}
-      get_vars utag xs FVmap Γ
-    {{ fun _ t s' =>
-         exists C S', 
-           fresh S' (fst s') /\
-           let '(xs', f) := t in
-           (forall σ,
-              f_eq σ (subst FVmap) ->
-              project_vars Scope Funs σ Γ FVs S xs xs' C S') /\
-           Forall2 (fun x x' => (subst FVmap) x = x') xs' xs' /\
-           is_exp_ctx f C }}.
-  Proof.
-    intros Hb1 Hb2 Hfv. eapply pre_post_mp_l.
-    revert S Hb1 Hb2 Hfv. induction xs; intros S Hb1 Hb2 Hfv. 
-    - eapply return_triple. intros [x' d'] _ Hf.
-      eexists Hole_c. repeat eexists; eauto.
-      constructor.
-    - eapply pre_post_mp_r. eapply bind_triple.
-      + eapply get_var_project_var_sound; eauto.
-        intros x Hin. eapply Hb1. 
-        inv Hin. constructor. eauto.
-      + intros [[x tau] f] [x' d']. eapply pre_eq_state.
-        intros [x'' d''] [C [S' [Hf [Hproj [Hsub Hctx]]]]].
-        eapply pre_post_mp_l. eapply bind_triple.
-        eapply (IHxs S'); eauto.
-        intros y Hin. eapply Hb1. 
-        constructor 2. eassumption.
-        intros z Hin. eapply Hb2. inversion Hin; eauto.
-        left. eapply project_var_free_set_Included. eapply Hproj.
-        reflexivity. eassumption.
-        intros [xs' f'] [x''' d''']. eapply return_triple. 
-        intros [x'''' d''''] Hyp Heq'. inversion Heq'.
-        destruct Hyp as [C' [S'' [Hf' [Hproj' [Hsub'  Hctx']]]]]; eauto.
-        now rewrite <- H0; eauto.
-        exists (comp_ctx_f C C'), S''.
-        split; [ eassumption |].
-        split. intros σ Heq. econstructor. eapply Hproj. eassumption.
-        eapply Hproj'. eassumption.
-        split. 
-        * constructor; eauto.
-        * intros e. rewrite <- app_ctx_f_fuse. congruence.
-  Qed.
-
-  (** Spec for [get_vars_with_types] *)
-  Lemma get_vars_with_types_project_vars_sound Scope Funs Γ FVs FVmap S xs :
-    binding_in_map (FromList xs) FVmap ->
-    binding_not_in_map (Union _ S (Singleton _ Γ)) FVmap ->
-    FVmap_inv FVmap Scope Funs FVs ->
-    {{ fun s => fresh S (fst s) }}
-      get_vars_with_types utag xs FVmap Γ
-    {{ fun _ t s' =>
-         exists C S', 
-           fresh S' (fst s') /\
-           let '(xs', _, f) := t in
-           (forall σ,
-              f_eq σ (subst FVmap) ->
-              project_vars Scope Funs σ Γ FVs S xs xs' C S') /\
-           Forall2 (fun x x' => (subst FVmap) x = x') xs' xs' /\
-           is_exp_ctx f C }}.
-  Proof.
-    intros Hb1 Hb2 Hfv. eapply pre_post_mp_l.
-    revert S Hb1 Hb2 Hfv. induction xs; intros S Hb1 Hb2 Hfv. 
-    - eapply return_triple. intros [x' d'] _ Hf.
-      eexists Hole_c. repeat eexists; eauto. constructor.
-    - eapply pre_post_mp_r. eapply bind_triple.
-      + eapply get_var_project_var_sound; eauto.
-        intros x Hin. eapply Hb1. 
-        inv Hin. constructor. eauto.
-      + intros [[x tau] f] [x' d']. eapply pre_eq_state.
-        intros [x'' d''] [C [S' [Hf [Hproj [Hsub Hctx]]]]].
-        eapply pre_post_mp_l. eapply bind_triple.
-        eapply (IHxs S'); eauto.
-        intros y Hin. eapply Hb1. 
-        constructor 2. eassumption.
-        intros z Hin. eapply Hb2. inversion Hin; eauto.
-        left. eapply project_var_free_set_Included. eapply Hproj.
-        reflexivity. eassumption.
-        intros [[xs' ts'] f'] [x''' d''']. eapply return_triple. 
-        intros [x'''' d''''] Hyp Heq. inversion Heq.
-        destruct Hyp as [C' [S'' [Hf' [Hproj' [Hsub' Hctx']]]]]; eauto.
-        now rewrite <- H0; eauto.
-        exists (comp_ctx_f C C'), S''.
-        split; [ eassumption |].
-        split. intros σ Hfeq. econstructor. eapply Hproj. eassumption.
-        eapply Hproj'. eassumption.
-        split. 
-        * constructor; eauto.
-        * intros e. rewrite <- app_ctx_f_fuse. congruence.
-  Qed.
-
-  Lemma subst_BoundVar_f_eq FVmap x t :
-    f_eq ((subst FVmap) {x ~> x}) (subst (M.set x (BoundVar t) FVmap)).
-  Proof.  
-    intros x'. unfold subst, extend. rewrite M.gsspec.
-    destruct (Coqlib.peq x' x). now eauto.
-    reflexivity. 
-  Qed.
-
-  Definition new_function_names FVmap : Ensemble var :=
-    fun x => exists y t1 t2, M.get y FVmap = Some (MRFun x t1 t2).
-
-  Lemma not_In_new_function_names_injective FVmap f:
-    ~ In _ (new_function_names FVmap) f ->
-    injective (subst FVmap) ->
-    injective ((subst FVmap) {f ~> f}).
-  Proof.
-    intros Hc Hinj x x' Heq. unfold extend in *.
-    destruct (Coqlib.peq x x'); eauto.
-    destruct (Coqlib.peq x f); eauto.
-    - destruct (Coqlib.peq x' f); try congruence.
-      exfalso. eapply Hc. 
-      eexists x'. unfold subst in Heq.
-      destruct (M.get x' FVmap) eqn:Heq'; eauto; try congruence.
-      subst. destruct v; try congruence.
-      eauto.
-    - destruct (Coqlib.peq x' f); [| now eauto ].
-      exfalso. eapply Hc. 
-      eexists x. unfold subst in Heq.
-      destruct (M.get x FVmap) eqn:Heq'; eauto; try congruence.
-      subst. destruct v; try congruence.
-      eauto.
-  Qed.
-
-  Lemma Disjoint_free_set FVmap Scope Funs FVs S :
-    binding_not_in_map S FVmap ->
-    FVmap_inv FVmap Scope Funs FVs ->
-    Disjoint _ S (Union var Scope
-                        (Union var Funs (FromList FVs))).
-  Proof.             
-    intros Hb [Hinv1 [Hinv2 Hinv3]].
-    constructor. intros x Hc. inv Hc. 
-    assert (Hdec1 : Decidable Scope).
-    { eapply Decidable_Same_set.
-      apply Same_set_sym. eassumption.
-      constructor. intros x'. destruct (M.get x' FVmap).
-      - destruct v; eauto;
-        right; intros [t' Hc]; congruence. 
-      - right. intros [t' Hc]. congruence. }
-    assert (Hdec2 : Decidable (Setminus _ Funs Scope)).
-    { eapply Decidable_Same_set.
-      apply Same_set_sym. eassumption.
-      constructor. intros x'. destruct (M.get x' FVmap).
-      - destruct v; eauto;
-        right; intros [y [t' [t'' Hc]]]; congruence. 
-      - right. intros [y [t' [t'' Hc]]]; congruence. }
-    destruct Hdec1, Hdec2.
-    destruct (Dec x). 
-    - eapply Hinv1 in H1. destruct H1 as [t Heq].
-      rewrite Hb in Heq; eauto. congruence.
-    - destruct (Dec0 x).
-      + eapply Hinv2 in H2. destruct H2 as [y [t [t' Heq]]].
-        rewrite Hb in Heq; eauto. congruence.
-      + inv H0; try contradiction.
-        inv H3. eapply H2; constructor; eauto.
-        unfold In, FromList in H0.        
-        edestruct In_nthN as [N Hnth]; [ eassumption |].
-        edestruct Hinv3 as [[t H'] _].
-        repeat split; eauto. intros Hin. eapply H2; constructor; eauto.
-        rewrite Hb in H'; eauto. congruence.
-  Qed.
-  
-  Lemma binding_not_in_map_antimon (A : Type) (S S' : Ensemble M.elt) (rho : M.t A):
-    Included M.elt S' S -> binding_not_in_map S rho -> binding_not_in_map S' rho.
-  Proof. 
-    intros Hin Hb x Hin'. eauto.
-  Qed.
-
-  Lemma binding_not_in_map_set_not_In_S {A} S map x (v : A) :
-    binding_not_in_map S map ->
-    ~ In _ S x ->
-    binding_not_in_map S (M.set x v map). 
-  Proof. 
-    intros HB Hnin x' Hin.
-    rewrite M.gsspec. destruct (Coqlib.peq x' x); subst; try contradiction. 
-    eauto. 
-  Qed.
-
-  Lemma new_function_names_set_BoundVar FVmap x t :
-    Included _ (new_function_names (M.set x (BoundVar t) FVmap)) (new_function_names FVmap).
-  Proof.
-    unfold new_function_names. intros x' [y [t' [t'' Hin]]].
-    rewrite M.gsspec in Hin. destruct (Coqlib.peq y x); try congruence.  
-    eauto.
-  Qed.
-
-  Import MonadNotation.
-
-  Transparent bind ret.
-
-  (** This identity is very useful to make the computation of the IH to appear
-      as a subcomputation in the goal *)
-  Lemma st_eq_Ecase {S} m1 (m2 : state S (var * type * (exp -> exp))) y :
-    st_eq
-      (ys <- m1 ;; 
-       ys' <- ret (y :: ys) ;;
-       t1 <- m2 ;;
-       let '(x, _ , f) := t1 in
-       ret (Ecase x ys', f))
-      (fe <- (ys <- m1 ;;
-             t1 <- m2 ;;
-             let '(x, _, f1) := t1 in    
-             ret (Ecase x ys, f1)) ;;
-       match fe with
-         | (Ecase x ys, f) =>
-           ret (Ecase x (y :: ys), f)
-         | _ => ret fe
-       end).
-  Proof.
-    unfold pbind, ret.
-    intros s. simpl. destruct (runState m1 s).
-    destruct (runState m2 s0). destruct p as [[x tau] f].
-    reflexivity.
-  Qed.
-
-  Opaque bind ret.
-
-  Lemma get_typeinfo_preserves_prop tau P :
-    {{ fun s => P (fst s) }} get_typeinfo tau {{ fun _ _ s => P (fst s) }}.
-  Proof.
-    eapply pre_post_mp_l. eapply bind_triple. eapply get_triple.
-    intros [x t] [x' t'].
-    destruct (TDict.get tau t); eapply return_triple;
-    intros [x'' t''] H HP; inv H; inv H0; inv H1; eauto.
-  Qed.
-
-  Lemma set_typeinfo_preserves_prop t P :
-    {{ fun s => P (fst s) }} set_typeinfo t {{ fun _ _ s => P (fst s) }}.
-  Proof.
-    eapply pre_post_mp_l. eapply bind_triple. eapply get_triple.
-    intros [x d] [x' d'].
-    destruct (TDict.hash t d).
-    eapply pre_post_mp_l. eapply bind_triple. eapply put_triple.
-    intros u [x'' d'']. eapply return_triple.
-    intros [x''' t'''] H1 [H2 H3] HP; inv H1; inv H2; inv H3; eauto.
-  Qed.
-  
-  Instance FVmap_inv_Scope_Proper :
-    Proper (Logic.eq ==> Same_set var ==> Logic.eq ==> Logic.eq ==> iff) FVmap_inv.
-  Proof. 
-    intros M1 M2 Heq1 S1 S2 Heq2 S3 S4 Heq3 l1 l2 Heq4; subst; split; intros [H1 [H2 H3]].
-    - (split; [| split ]); try rewrite <- Heq2; eauto. 
-      split. intros [Hnth [Hnin1 Hnin2]]. eapply H3. repeat split; eauto.
-      now rewrite Heq2.
-      intros H. rewrite <- Heq2. eapply H3. eassumption. 
-    - (split; [| split ]); try rewrite Heq2; eauto. 
-      split. intros [Hnth [Hnin1 Hnin2]]. eapply H3. repeat split; eauto.
-      now rewrite <- Heq2.
-      intros H. rewrite Heq2. eapply H3. eassumption. 
-  Qed.
-
-  Instance FVmap_inv_Funs_Proper :
-    Proper (Logic.eq ==> Logic.eq ==> Same_set var ==> Logic.eq ==> iff) FVmap_inv.
-  Proof. 
-    intros M1 M2 Heq1 S1 S2 Heq2 S3 S4 Heq3 l1 l2 Heq4; subst; split; intros [H1 [H2 H3]].
-    - (split; [| split ]); try rewrite <- Heq3; eauto.
-      split. intros [Hnth [Hnin1 Hnin2]]. eapply H3. repeat split; eauto.
-      now rewrite Heq3.
-      intros H. rewrite <- Heq3. eapply H3. eassumption. 
-    - (split; [| split ]); try rewrite Heq3; eauto. 
-      split. intros [Hnth [Hnin1 Hnin2]]. eapply H3. repeat split; eauto.
-      now rewrite <- Heq3.
-      intros H. rewrite Heq3. eapply H3. eassumption. 
-  Qed.
-
-  Lemma FVmapInv_add_params FVmap xs ts Scope Funs FVs :
-    FVmap_inv FVmap Scope Funs FVs ->
-    FVmap_inv (add_params xs ts FVmap) (Union _ Scope (FromList xs)) Funs FVs. 
-  Proof. 
-    revert FVmap ts Scope. induction xs; intros FVmap ts Scope Hinv.
-    - rewrite FromList_nil, Union_Empty_set_l. eauto.
-    - rewrite FromList_cons.
-      rewrite Union_assoc; rewrite Union_sym with (s2 := Singleton M.elt a), <- Union_assoc. 
-      destruct ts; eapply FVmap_inv_set_bound; eauto.
-  Qed.
-
-  Lemma binding_in_map_add_params S FVmap xs ts :
-    binding_in_map S FVmap ->
-    binding_in_map (Union _ S  (FromList xs)) (add_params xs ts FVmap).
-  Proof.
-    revert S FVmap ts. induction xs; intros S FVmap ts Hb.
-    - intros x. rewrite FromList_nil, Union_Empty_set_l. eauto.
-    - intros x. rewrite FromList_cons.
-      rewrite Union_sym with (s2 := FromList xs), Union_assoc.
-      simpl. destruct ts; eapply binding_in_map_set; eauto. 
-  Qed.
-
-  Lemma binding_not_in_map_add_params S FVmap xs ts :
-    binding_not_in_map S FVmap ->
-    Disjoint _ S (FromList xs) ->
-    binding_not_in_map S (add_params xs ts FVmap).
-  Proof.
-    revert S FVmap ts. induction xs; intros S FVmap ts Hb Hd.
-    - eauto.
-    - rewrite FromList_cons in Hd.
-      destruct ts; simpl; eapply binding_not_in_map_set_not_In_S; eauto.
-      + eapply IHxs. eassumption.
-        constructor. intros x Hc. inv Hc. eapply Hd. now constructor; eauto.
-      + intros Hc. eapply Hd. eauto.
-      + eapply IHxs. eassumption.
-        constructor. intros x Hc. inv Hc. eapply Hd. now constructor; eauto.
-      + intros Hc. eapply Hd. eauto.
-  Qed.
-
-  Lemma new_function_names_add_params FVmap xs ts :
-    Included  _ (new_function_names (add_params xs ts FVmap)) (new_function_names FVmap).
-  Proof.
-    revert FVmap ts. induction xs; intros FVmap ts; simpl. 
-    - apply Included_refl.
-    - destruct ts;
-      (eapply Included_trans;
-       [ eapply new_function_names_set_BoundVar | eapply IHxs ]).
-  Qed.
-
-  Lemma injective_add_params FVmap xs ts :
-    Disjoint _ (new_function_names FVmap) (FromList xs) ->
-    injective (subst FVmap) ->
-    injective (subst (add_params xs ts FVmap)).
-  Proof. 
-    revert FVmap ts. induction xs; intros FVmap ts Hd Hinj.
-    - eassumption. 
-    - simpl. destruct ts; rewrite <- subst_BoundVar_f_eq;
-      eapply not_In_new_function_names_injective.
-      + intros Hc. eapply Hd. constructor.
-        eapply new_function_names_add_params. eassumption. 
-        rewrite FromList_cons. eauto.
-      + eapply IHxs. constructor. intros x Hin. 
-        inv Hin. eapply Hd. constructor; eauto.
-        rewrite FromList_cons. eauto.
-        eassumption.
-      + intros Hc. eapply Hd. constructor.
-        eapply new_function_names_add_params. eassumption. 
-        rewrite FromList_cons. eauto.
-      + eapply IHxs. constructor. intros x Hin. 
-        inv Hin. eapply Hd. constructor; eauto.
-        rewrite FromList_cons. eauto.
-        eassumption.
-  Qed.
-
-  Lemma construct_lst_injection_add_params FVmap xs ts :
-    Disjoint _ (new_function_names FVmap) (FromList xs) ->
-    injective (subst FVmap) ->
-    exists f,
-      f_eq f (subst (add_params xs ts FVmap)) /\
-      construct_lst_injection (subst FVmap) xs xs f.
-  Proof.
-    revert FVmap ts. induction xs; intros FVmap ts Hd Hinj.  
-    - eexists. split. simpl. reflexivity. constructor.
-    - assert (Hinj' : injective (subst (add_params (a :: xs) ts FVmap))).
-      { apply injective_add_params; eauto. }
-      rewrite FromList_cons in Hd.
-      destruct ts; edestruct IHxs as [f [Heq Hinj'']]. 
-      + eapply Disjoint_Included_r; [ | eassumption ].
-        now apply Included_Union_r. 
-      + eassumption.
-      + eexists (f {a ~> a}). split. 
-        simpl. rewrite Heq. eapply subst_BoundVar_f_eq.
-        constructor. eassumption. 
-        rewrite Heq. simpl in Hinj'. rewrite subst_BoundVar_f_eq.
-        eassumption.
-      + eapply Disjoint_Included_r; [ | eassumption ].
-        now apply Included_Union_r. 
-      + eassumption.
-      + eexists (f {a ~> a}). split. 
-        simpl. rewrite Heq. eapply subst_BoundVar_f_eq.
-        constructor. eassumption. 
-        rewrite Heq. simpl in Hinj'. rewrite subst_BoundVar_f_eq.
-        eassumption.
-  Qed.
-          
-  Lemma FVmap_inv_empty :
-    FVmap_inv (Maps.PTree.empty VarInfo) (Empty_set M.elt) (Empty_set M.elt) [].
-  Proof.
-    repeat split; (try now intros Hc; inv Hc); (try now intros x Hc; inv Hc). 
-    intros x Hx. destruct Hx as [t Hget]. rewrite M.gempty in Hget. now inv Hget.
-    destruct H as [x' [t [t' Hget]]]. rewrite M.gempty in Hget. now inv Hget.
-    destruct H as [t Hget]. rewrite M.gempty in Hget. now inv Hget.
-  Qed.
-  
-  Lemma nthN_app {A} (l1 l2 : list A) N :
-    (nthN (l1 ++ l2) N = nthN l1 N) \/
-    (nthN (l1 ++ l2) N = nthN l2 (N - N.of_nat (length l1))%N /\ (N.of_nat (length l1) <= N)%N).
-  Proof. 
-    revert N; induction l1; intros N.
-    - right. rewrite app_nil_l, N.sub_0_r. split; eauto. simpl. zify; omega.
-    - destruct N; [now eauto |].
-      destruct (IHl1 ((N.pos p)-1)%N) as [H1 | [H2 H3]].
-      now eauto.
-      replace (N.of_nat (length (a :: l1))) with (1 + N.of_nat (length l1))%N.
-      replace (N.pos p - (1 + N.of_nat (length l1)))%N with
-      (N.pos p - 1 - N.of_nat (length l1))%N.
-      right. split. now eauto. zify. omega. 
-      zify; omega. 
-      simpl (length _). rewrite Nnat.Nat2N.inj_succ.
-      zify. omega. 
-  Qed.
-  
-  Lemma nthN_is_Some_length {A} (l : list A) N x :
-    nthN l N = Some x ->
-    (N < N.of_nat (length l))%N.
-  Proof. 
-    revert N. induction l; intros N Heq.
-    - inv Heq. 
-    - destruct N. inv Heq.
-      unfold length. rewrite Nnat.Nat2N.inj_succ. zify. omega. 
-      assert (Hlt : ((N.pos p)-1 < N.of_nat (length l))%N) by eauto.
-      simpl (length _). rewrite Nnat.Nat2N.inj_succ.
-      zify. omega. 
-  Qed.
-  
-  Lemma nthN_app_geq {A} (l1 l2 : list A) N :
-    (N.of_nat (length l1) <= N)%N ->
-    nthN (l1 ++ l2) N = nthN l2 (N - N.of_nat (length l1))%N.
-  Proof.
-    revert N. induction l1; intros N Heq.
-    - simpl. rewrite N.sub_0_r. reflexivity.
-    - simpl length in *. 
-      destruct N. 
-      zify. omega.
-      rewrite Nnat.Nat2N.inj_succ.
-      rewrite <- N.add_1_l, N_as_DT.sub_add_distr. 
-      rewrite <- IHl1.
-      reflexivity. zify. omega. 
-  Qed.
-  
-  Lemma nthN_is_Some_app {A} (l1 l2 : list A) N x :
-    nthN l1 N = Some x ->
-    nthN (l1 ++ l2) N = Some x.
-  Proof.
-    revert N. induction l1; intros N Heq.
-    - inv Heq.
-    - destruct N. inv Heq. reflexivity.
-      simpl. eauto.
-  Qed.
-  
-  Lemma FVmap_inv_set_free_var FVmap Scope Funs FVs x n t:
-    FVmap_inv FVmap Scope Funs FVs ->
-    N.of_nat (length FVs) = n ->
-    ~ In _ Scope x -> ~ In  _ Funs x -> ~ List.In x FVs ->
-    FVmap_inv (Maps.PTree.set x (FVar n t) FVmap) Scope Funs (FVs ++ [x]). 
-  Proof.  
-    intros [H1 [H2 H3]] Hlen Hnin1 Hnin2.
-    split; [| split ]. 
-    - split.
-      + intros x' Hin. assert (Hin' := Hin).
-        eapply H1 in Hin. edestruct Hin as [t' Heq].
-        destruct (Coqlib.peq x' x).
-        subst; contradiction.
-        eexists. rewrite M.gso; eauto.
-      + intros x' [t' Hget]. eapply H1. 
-        rewrite M.gsspec in Hget. destruct (Coqlib.peq x' x).
-        subst; congruence.
-        now eauto.
-    - split.
-      + intros x' Hin. assert (Hin' := Hin). inv Hin'. 
-        eapply H2 in Hin. edestruct Hin as [y [t1 [t2 Heq]]].
-        destruct (Coqlib.peq x' x).
-        subst; contradiction.
-        eexists. rewrite M.gso; eauto.
-      + intros x' [y [t1 [t2 Hget]]]. eapply H2. 
-        rewrite M.gsspec in Hget. destruct (Coqlib.peq x' x).
-        subst; congruence.
-        now eauto.
-    - intros N x'. split.
-      + intros [Hnth [Hnin1' Hnin2']].
-        destruct (nthN_app FVs [x] N) as [Hn | [Hn Hlen']].
-        * destruct (Coqlib.peq x' x); subst.
-          exfalso. eapply H. eapply nthN_In. rewrite <- Hnth. now eauto.
-          edestruct H3 as [[t' Hget] _].
-          repeat split; eauto. rewrite <- Hnth. now eauto.
-          eexists. now rewrite M.gso; eauto.
-        * subst. rewrite Hnth in Hn. eapply nthN_is_Some_length in Hnth.
-          rewrite app_length in Hnth. simpl length in *.
-          destruct (N - N.of_nat (length FVs))%N eqn:Heq; simpl in Hn; try congruence.
-          inv Hn. eexists. rewrite M.gss; eauto.
-          repeat f_equal. zify. omega. 
-      + subst. intros [t' Hget].
-        rewrite M.gsspec in Hget. destruct (Coqlib.peq x' x).
-        * subst. inv Hget. repeat split; eauto.
-          rewrite nthN_app_geq. rewrite N.sub_diag. reflexivity. 
-          zify; omega. 
-        * edestruct H3 as [_ [H1' [H2' H3']]].
-          now eexists; eauto.
-          repeat split; eauto. apply nthN_is_Some_app. eassumption.
-  Qed.
-
-  Lemma make_env_spec fv FVmap_o Γ_n Γ_o Scope Funs FVs S :
-    binding_in_map (FromList (PS.elements fv)) FVmap_o ->
-    binding_not_in_map (Union M.elt S (Singleton M.elt Γ_o)) FVmap_o ->
-    FVmap_inv FVmap_o Scope Funs FVs ->
-    {{ fun s => fresh S (fst s) }}
-      make_env utag env_tag fv (Maps.PTree.empty VarInfo) FVmap_o Γ_n Γ_o 
-    {{ fun s t  s' =>
-         let '(_, FVmap_n, f) := t in
-         exists C S' FVs' tau t,
-           fresh S' (fst s') /\
-           (forall σ, f_eq σ (subst FVmap_o) ->
-                 project_vars Scope Funs σ Γ_o FVs S (PS.elements fv) FVs' C S') /\
-           Forall2 (fun (x : M.elt) (x' : var) => subst FVmap_o x = x')
-                   FVs' FVs' /\
-           is_exp_ctx f (comp_ctx_f C (Econstr_c Γ_n tau t FVs' Hole_c)) /\
-           FVmap_inv FVmap_n (Empty_set _) (Empty_set _) (PS.elements fv)
-     }}.
-  Proof.
-    intros Hb1 Hb2 Minv. eapply bind_triple. 
-    - eapply get_vars_with_types_project_vars_sound; eauto.
-    - intros [[xs ts] f] s1.
-      eapply pre_existential. intros C1. eapply pre_existential. intros S'.
-      eapply pre_uncurry_r. intros [Hvars [Hall Hctx]].
-      eapply bind_triple. now eapply set_typeinfo_preserves_prop.
-      intros tau s2. eapply return_triple.
-      intros s3 Hf. do 6 eexists. eassumption. 
-      repeat (split; [ eassumption |]). split.
-      + intros e. rewrite Hctx. rewrite <- app_ctx_f_fuse.
-        f_equal. reflexivity.
-      + clear.
-        assert (He : FVmap_inv (Maps.PTree.empty VarInfo)
-                               (Empty_set M.elt) (Empty_set M.elt) (@nil PS.elt))
-          by apply FVmap_inv_empty.
-        assert (Hlen : N.of_nat (@length PS.elt []) = 0%N) by eauto.
-        assert (Hnin : forall x, List.In x (PS.elements fv) -> ~ List.In x (@nil PS.elt))
-          by (intros x H1 H2; inv H2).
-        assert (Hdup :  NoDupA eq (PS.elements fv)) by apply PS.elements_spec2w.
-        replace (PS.elements fv) with ([] ++ PS.elements fv) at 2 by reflexivity.
-        revert Hlen He Hnin Hdup. generalize (Maps.PTree.empty VarInfo) as FVmap_i.
-        generalize (@nil PS.elt). generalize 0%N. 
-        induction (PS.elements fv); intros n vars FVmap_i Hlen Hinv Hnin Hdup.
-        * rewrite app_nil_r. simpl. assumption.
-        * simpl. replace (vars ++ a :: l) with ((vars ++ [a]) ++ l).
-          eapply IHl. rewrite app_length. simpl. zify. omega. 
-          eapply FVmap_inv_set_free_var. now eauto. eassumption. 
-          now intros Hc; inv Hc. now intros Hc; inv Hc. 
-          eapply Hnin. constructor. reflexivity.
-          intros x Hin Hc. eapply Hnin.  
-          now constructor 2; eauto. inv Hdup.
-          apply Coqlib.in_app in Hc. inv Hc; eauto. inv H. 
-          exfalso. eapply H1. eapply In_InA. eauto. now eapply Pos.eq_equiv. 
-          eassumption. now inv H0. now inv Hdup.
-          rewrite <- app_assoc. reflexivity.
-  Qed.
-
-  Lemma subst_MRFun_f_eq (FVmap : VarInfoMap) (x x' : var) (t t': type) :
-    f_eq ((subst FVmap) {x ~> x'}) (subst (M.set x (MRFun x' t t') FVmap)).
-  Proof.
-    unfold subst. intros y. unfold extend.
-    rewrite M.gsspec. destruct (Coqlib.peq y x); eauto.
-  Qed.
-
-  Instance image_Proper {A B} : Proper (f_eq ==> Logic.eq ==> Same_set _) (@image A B).
-  Proof.
-    intros x1 x2 Heq s1 s2 Heq'; subst.
-    split; intros x [y1 [Hin Heq']]; subst;
-    eexists; eauto.
-  Qed.
-
-  Lemma make_full_closure_spec B FVmap_n FVmap_o Γ Scope Funs FVs FVs' typ S :
-    FVmap_inv FVmap_o Scope Funs FVs ->
-    FVmap_inv FVmap_n (Empty_set _) (Empty_set _) FVs' ->
-    {{ fun s => fresh S (fst s) }}
-      make_full_closure utag tag_bij unknown_type B FVmap_n FVmap_o Γ typ
-    {{ fun s t s' =>
-         let '(FVmap_n', FVmap_o', f) := t in
-         exists C σ S',
-           fresh S' (fst s') /\
-           make_closures B S id Γ C S' σ /\
-           f_eq σ (subst FVmap_n') /\
-           is_exp_ctx f C /\
-           FVmap_inv FVmap_o' (Union _ (name_in_fundefs B) Scope) Funs FVs /\
-           FVmap_inv FVmap_n' (Empty_set _) (name_in_fundefs B) FVs'
-     }}.
-  Proof.
-    revert FVmap_n FVmap_o Γ Scope Funs FVs FVs' typ S.
-    induction B; intros FVmap_n FVmap_o Γ Scope Funs FVs FVs' typ S Minv_o Minv_n.
-    - eapply bind_triple; [ now apply get_name_fresh |].
-      intros x s1. eapply pre_uncurry_l. intros Hx.
-      eapply bind_triple; [ eapply IHB; eassumption |].
-      intros [[FVmap_n' FVmap_o'] f] _.
-      eapply pre_existential. intros C.  eapply pre_existential. intros σ.
-      eapply pre_existential. intros S'.
-      eapply pre_uncurry_r. intros [Hclo [Hfeq [Hctx [Minv_o' Minv_n']]]].
-      eapply bind_triple; [ now apply get_typeinfo_preserves_prop |].
-      intros t_inf s2.
-      eapply bind_triple with
-      (post' := fun _ _ s =>  fresh S' (fst s)).
-      + destruct t_inf; try now apply return_triple. 
-        eapply bind_triple. now apply set_typeinfo_preserves_prop.
-        intros. eapply bind_triple. now apply set_typeinfo_preserves_prop.
-        intros. now apply return_triple. 
-      + intros [typ' typ''] _. apply return_triple. 
-        intros s3 Hf. do 3 eexists.
-        split. eassumption. 
-        split. econstructor. eassumption. eapply Hx. zify; omega.
-        split. setoid_rewrite <- subst_MRFun_f_eq.
-        eapply f_eq_extend; eauto.
-        split. intros e'. simpl. rewrite Hctx. reflexivity.
-        split.
-        simpl. rewrite <- Union_assoc. eapply FVmap_inv_set_bound. eassumption.
-        simpl. apply FVmap_inv_set_funs. now apply not_In_Empty_set.
-        eassumption. 
-    - eapply return_triple. intros s Hs. do 3 eexists.
-      split. eassumption. split. now constructor.
-      split.
-      intros x. unfold subst. destruct (M.get x FVmap_n) eqn:Heq; eauto.
-      destruct v; eauto. destruct Minv_n as [H1 [H2 H3]].
-      exfalso. rewrite Setminus_Empty_set in H2. eapply not_In_Empty_set.
-      eapply H2. now repeat eexists; eauto.
-      split. intros e. reflexivity.
-      split. rewrite Union_Empty_set_r. eassumption. 
-      eassumption. 
-  Qed.
-
-  Lemma image_extend_not_In f x x' S :
-    ~ In _ S x ->
-    Same_set _ (image (f {x ~> x'} ) S) (image f S).
-  Proof.    
-    intros Hnin.
-    split; intros y [y' [Hin Heq]]. rewrite extend_gso in Heq.
-    now eexists; eauto. intros Hc. subst. contradiction.
-    eexists; split; eauto. rewrite extend_gso. now eauto.
-    intros Hc. subst. contradiction.
-  Qed.
-
-  Definition feq_subdomain {A B} (f1 f2 : A -> B) S :=
-    forall x, In _ S x -> f1 x = f2 x.
-
-  Lemma exp_closure_conv_Closure_conv_sound :
-    (forall e Scope Funs Γ FVs FVmap S
-       (* The invariant the relates [FVmap] and [Scope], [Funs], [FV] *)
-       (Minv : FVmap_inv FVmap Scope Funs FVs)
-       (* [FVmap] contains all the free variables *)
-       (Hbin1 : binding_in_map (occurs_free e) FVmap)
-       (* [FVmap] does not contain the variables in [S] or [Γ] *)
-       (Hbin2 : binding_not_in_map (Union _ S (Singleton _ Γ)) FVmap)
-       (* [S] is disjoint with the free and bound variables of [e] and [Γ] *)
-       (HD1 : Disjoint _ S (Union _ (bound_var e)
-                                  (Union _ (occurs_free e) (Singleton _ Γ))))
-       (* The current environment argument is fresh *)
-       (HD2 : ~ In _ (Union _ (bound_var e) (occurs_free e)) Γ)
-       (* (* Τhe new function names in the substitution are fresh *) *)
-       (HD3 : Disjoint _ (image (subst FVmap) (Setminus _ Funs Scope))
-                       (Union _ (occurs_free e) (bound_var e))),
-       {{ fun s => True }}
-         exp_closure_conv utag env_tag tag_bij unknown_type e FVmap Γ
-       {{ fun s ef s' =>
-            fresh S (fst s) ->
-            exists C σ, is_exp_ctx (snd ef) C /\
-                   f_eq (subst FVmap) σ /\
-                   Closure_conversion Scope Funs σ Γ FVs e (fst ef) C /\
-                   fresh S (fst s')
-       }}) /\
-    (forall B FVmap Funs FVs S
-       (Minv : FVmap_inv FVmap (Empty_set _) Funs FVs)
-       (Hbin1 : binding_in_map (Union _ (occurs_free_fundefs B) (name_in_fundefs B)) FVmap)
-       (Hbin2 : binding_not_in_map S FVmap)
-       (HD1 : Disjoint _ S (Union _ Funs (Union _ (bound_var_fundefs B) (occurs_free_fundefs B))))
-       (HD2 : Disjoint _ (image (subst FVmap) Funs) (Union _ (bound_var_fundefs B) (occurs_free_fundefs B)))
-       (Hinc : Included _ (name_in_fundefs B) Funs),
-       {{ fun s => True }}
-         fundefs_closure_conv utag env_tag tag_bij unknown_type B FVmap
-       {{ fun s B' s' =>
-            fresh S (fst s) ->       
-            exists σ, Closure_conversion_fundefs Funs σ FVs B B' /\
-                 fresh S (fst s')
-       }}).
-  Proof.
-(*    eapply exp_def_mutual_ind; intros.
-    - eapply pre_post_mp_r. eapply bind_triple.
-      + eapply get_vars_project_vars_sound; [ | eassumption | eassumption ].
-        intros x Hx. eapply Hbin1. eauto.
-      + intros [xs f] s. eapply pre_eq_state.
-        intros [x'' d''] [C [S' [Hf [Hproj [Hsub  Hctx]]]]].
-        eapply pre_post_mp_l.
-        eapply bind_triple.
-        eapply H with (Scope := Union var (Singleton var v) Scope)
-                      (S := S')
-                      (FVmap := Maps.PTree.set v (BoundVar t) FVmap).
-        * eapply FVmap_inv_set_bound. eassumption. 
-        * eapply binding_in_map_antimon; [| eapply binding_in_map_set; eassumption ].
-          now eapply occurs_free_Econstr_Included.
-        * eapply binding_not_in_map_antimon.
-          apply Included_Union_compat. eapply project_vars_free_set_Included; eauto.
-          eapply Hproj. reflexivity. 
-          now apply Included_refl.
-          eapply binding_not_in_map_set_not_In_S. eassumption.  
-          intros Hc; inv Hc. now eapply HD1; eauto. inv H0; eapply HD2; eauto.
-        * rewrite bound_var_Econstr, occurs_free_Econstr in HD1.
-          eapply Disjoint_Included_l. eapply project_vars_free_set_Included.
-          eapply Hproj. reflexivity.
-          eapply Disjoint_Included_r; [| eassumption ]. rewrite <- Union_assoc.
-          apply Included_Union_compat. now apply Included_refl.
-          rewrite Union_assoc.
-          apply Included_Union_compat; [| now apply Included_refl ].
-          rewrite Union_sym, <- Union_assoc. eapply Included_Union_mon_r.
-          rewrite <- (@Union_Setminus _ _ _ _). now apply Included_Union_l.
-        * intros Hc. inv Hc; eapply HD2; eauto.
-          rewrite bound_var_Econstr, occurs_free_Econstr.
-          destruct (Coqlib.peq Γ v); subst;  eauto.
-          right. right. constructor; eauto. intros Hc; inv Hc. congruence.
-        * rewrite <- subst_BoundVar_f_eq. rewrite image_extend_not_In.
-          eapply Disjoint_Included_l. eapply image_monotonic.
-          eapply Included_Setminus_compat. now eapply Included_refl.
-          now apply Included_Union_r.
-          eapply Disjoint_Included_r; [| eassumption].
-          rewrite bound_var_Econstr, occurs_free_Econstr.
-          rewrite <- !Union_assoc. apply Included_Union_mon_r.
-          rewrite !Union_assoc, (Union_sym _ (Singleton var v)), !Union_assoc.
-          apply Included_Union_compat; [| now apply Included_refl ].
-          rewrite (@Setminus_Union_Included _ _ _ _ _).
-          now apply Included_Union_r. now apply Included_refl.
-          intros Hc. inv Hc. eauto.
-        * intros e' s'. eapply return_triple. intros s'' Hf' Hcc. subst.
-          edestruct (Hf' Hf) as [C' [σ [Hctx' [Hfeq [Hcc Hf'']]]]]; eauto.
-          do 2 eexists. split. eapply Hctx. split.
-          rewrite <- f_eq_extend_same, subst_BoundVar_f_eq. eassumption.
-          unfold subst. rewrite Hbin2. reflexivity. eassumption.
-          Focus 2.
-          split. simpl. rewrite Hctx'. econstructor. 
-          rewrite !Union_assoc. eapply Disjoint_sym. eapply Disjoint_Union; eapply Disjoint_sym. 
-          rewrite <- Union_assoc. eapply Disjoint_free_set. ; [| eassumption ].
-          eapply binding_not_in_map_antimon; [| eassumption ]. now apply Included_Union_l.
-          eapply Disjoint_Included_r; [| eassumption ]. do 2 apply Included_Union_mon_r.
-          now apply Included_refl.
-          eassumption. eassumption. 
-          split. eassumption. constructor. eassumption.
-          eapply not_In_new_function_names_injective.
-          intros Hc. eapply HD3; eauto. eassumption.
-          rewrite subst_BoundVar_f_eq. rewrite HC''. now eauto.
-          eapply fresh_monotonic. now eapply project_vars_free_set_Included; eauto.
-          eassumption.
-    - eapply pre_post_mp_r. eapply bind_triple with (post' := fun _ l i => l = [] /\ fresh S (fst i)).
-      + eapply return_triple; eauto. 
-      + intros pats' s2.
-        eapply bind_triple.
-        * eapply frame_rule. eapply get_var_project_var_sound; eauto.
-          intros x Hx. eapply Hbin1. rewrite occurs_free_Ecase_nil. eassumption.
-        * intros [[x tau] f] s. eapply return_triple.
-          intros s' [Heq [C [C' [S' [Hf [Hproj [Hsub [Halpha Hctx]]]]]]]]. rewrite Heq.
-          eexists. split; eauto. split. econstructor. eexists. split. econstructor.
-          rewrite !Union_assoc. eapply Disjoint_sym. eapply Disjoint_Union; eapply Disjoint_sym. 
-          rewrite <- Union_assoc. eapply Disjoint_free_set; [| eassumption ].
-          eapply binding_not_in_map_antimon; [| eassumption ]. now apply Included_Union_l.
-          eapply Disjoint_Included_r; [| eassumption ]. do 2 apply Included_Union_mon_r.
-          now apply Included_refl.
-          eassumption. now constructor.
-          split. eassumption. now constructor.
-          eapply fresh_monotonic. now eapply project_var_free_set_Included; eauto.
-          eassumption.
-    - unfold exp_closure_conv. setoid_rewrite assoc.
-      eapply bind_triple.
-      + eapply H; [ eassumption | eassumption | | eassumption | | | ].
-        * eapply binding_in_map_antimon; [| eassumption ].
-          eapply occurs_free_Ecase_Included. now constructor.
-        * eapply Disjoint_Included_r; [| eassumption ].
-          apply Included_Union_compat.
-          rewrite bound_var_Ecase_cons. now apply Included_Union_l.
-          rewrite occurs_free_Ecase_cons.
-          apply Included_Union_compat. now apply Included_Union_l.
-          now apply Included_refl.
-        * intros Hc. apply HD2.
-          rewrite bound_var_Ecase_cons, occurs_free_Ecase_cons.
-          inv Hc; eauto.
-        * eapply Disjoint_Included_r; [| eassumption ].
-          apply Included_Union_compat.
-          rewrite occurs_free_Ecase_cons. now apply Included_Union_l.
-          rewrite bound_var_Ecase_cons. now apply Included_Union_l.
-      + intros [e' f'] s'.  simpl. setoid_rewrite assoc. simpl.
-        setoid_rewrite st_eq_Ecase. 
-        eapply pre_post_mp_l. eapply bind_triple. 
-        eapply H0 with (FVmap := FVmap) (Γ := Γ);
-          [ eassumption | eassumption | | eassumption | | | ].
-        * eapply binding_in_map_antimon; [| eassumption ].
-          rewrite occurs_free_Ecase_cons. apply Included_Union_mon_r.
-          now apply Included_Union_r.
-        * eapply Disjoint_Included_r; [| eassumption ].
-          apply Included_Union_compat.
-          rewrite bound_var_Ecase_cons. now apply Included_Union_r.
-          rewrite occurs_free_Ecase_cons.
-          apply Included_Union_compat. apply Included_Union_mon_r.
-          now apply Included_Union_r.
-          now apply Included_refl.
-        * intros Hc. apply HD2.
-          rewrite bound_var_Ecase_cons, occurs_free_Ecase_cons.
-          inv Hc; eauto.
-        * eapply Disjoint_Included_r; [| eassumption ].
-          apply Included_Union_compat.
-          rewrite occurs_free_Ecase_cons. apply Included_Union_mon_r.
-          now apply Included_Union_r.
-          rewrite bound_var_Ecase_cons. now apply Included_Union_r.
-        * intros [e'' f s''].   
-          edestruct e''; eapply return_triple; intros s''' Hcc1 Hcc2 Hf;
-          edestruct (Hcc2 Hf) as [C2 [Hctx1 [[e2 [C2' [Hc2' [Ha2 Ha2']]]] Hf'']]];
-          edestruct (Hcc1 Hf'') as [C1 [Hctx2 [[e1 [C1' [Hcc1' [Ha1 Ha1']]]] Hf''']]];
-          inv Hcc1'; inv Ha1'.
-          eexists. repeat split.
-          eassumption.
-          repeat eexists.
-          eapply CC_Ecase with (pats' := (c, (C2' |[ e2 ]|)) :: pats'); eauto.
-          econstructor; [| eassumption ]. split; eauto. repeat eexists; eauto.
-          eassumption. econstructor; eauto.
-          econstructor; [| eassumption ]. split; eauto.
-          rewrite Hctx1. now eauto.
-          eassumption.
-    - eapply pre_post_mp_r. eapply bind_triple.
-      + eapply get_var_project_var_sound; [ eassumption | | eassumption | eassumption ].
-        intros x Hx. inv Hx. eapply Hbin1. eauto.
-      + intros [[x tau] f] s. eapply pre_eq_state.
-        intros [x'' d''] [C [C' [S' [Hf [Hproj [Hsub [Halpha Hctx]]]]]]].
-        eapply pre_post_mp_l.
-        eapply bind_triple.
-        eapply H with (Scope := Union var (Singleton var v) Scope)
-                      (S := S')
-                      (FVmap := Maps.PTree.set v (BoundVar t) FVmap).
-        * eapply FVmap_inv_set_bound. eassumption. 
-        * rewrite <- subst_BoundVar_f_eq. eapply not_In_new_function_names_injective.
-          intros Hc. eapply HD3. now eauto. assumption.
-        * eapply binding_in_map_antimon; [| eapply binding_in_map_set; eassumption ].
-          now eapply occurs_free_Eproj_Included.
-        * eapply binding_not_in_map_antimon.
-          apply Included_Union_compat. now eapply project_var_free_set_Included; eauto.
-          now apply Included_refl.
-          eapply binding_not_in_map_set_not_In_S. eassumption. clear Hsub.
-          intros Hc; inv Hc. now eapply HD1; eauto. inv H0; eapply HD2; eauto.
-        * rewrite bound_var_Eproj, occurs_free_Eproj in HD1.
-          eapply Disjoint_Included_l. now eapply project_var_free_set_Included; eauto.
-          eapply Disjoint_Included_r; [| eassumption ]. rewrite <- Union_assoc.
-          apply Included_Union_compat. now apply Included_refl.
-          rewrite Union_assoc.
-          apply Included_Union_compat; [| now apply Included_refl ].
-          rewrite Union_sym, <- Union_assoc. eapply Included_Union_mon_r.
-          rewrite <- (@Union_Setminus _ _ _ _). now apply Included_Union_l.
-        * intros Hc. clear Hsub. inv Hc; eapply HD2; eauto.
-          rewrite bound_var_Eproj, occurs_free_Eproj.
-          destruct (Coqlib.peq Γ v); subst;  eauto.
-          right. right. constructor; eauto. intros Hc; inv Hc. congruence.
-        * eapply Disjoint_Included_l;[ now apply new_function_names_set_BoundVar | ].
-          eapply Disjoint_Included_r; [| eassumption ].
-          rewrite bound_var_Eproj, occurs_free_Eproj.
-          rewrite <- !Union_assoc. apply Included_Union_mon_r.
-          rewrite !Union_assoc, (Union_sym _ (Singleton var v)), !Union_assoc.
-          apply Included_Union_compat; [| now apply Included_refl ].
-          rewrite (@Setminus_Union_Included _ _ _ _ _).
-          now apply Included_Union_r. now apply Included_refl.
-        * intros e' s'. eapply return_triple. intros s'' Hf' Hcc. subst s'.
-          edestruct (Hf' Hf) as [C'' [HC'' [[e'' [Ce [Hcc [Ha1 Ha2]]]] Hf'']]]; eauto. 
-          exists C'. split. now eauto. split. do 2 eexists. split.
-          econstructor.
-          rewrite !Union_assoc. eapply Disjoint_sym. eapply Disjoint_Union; eapply Disjoint_sym. 
-          rewrite <- Union_assoc. eapply Disjoint_free_set; [| eassumption ].
-          eapply binding_not_in_map_antimon; [| eassumption ]. now apply Included_Union_l.
-          eapply Disjoint_Included_r; [| eassumption ]. do 2 apply Included_Union_mon_r.
-          now apply Included_refl.
-          eassumption. eassumption. 
-          split. eassumption. constructor. eassumption.
-          eapply not_In_new_function_names_injective.
-          intros Hc. eapply HD3; eauto. eassumption.
-          rewrite subst_BoundVar_f_eq. rewrite HC''. now eauto.
-          eapply fresh_monotonic. now eapply project_var_free_set_Included; eauto.
-          eassumption.
-    - admit.
-    - eapply pre_post_mp_r. eapply bind_triple.
-      + eapply get_var_project_var_sound; [ eassumption | | eassumption | eassumption ].
-        intros x Hx. eapply Hbin1. inv Hx. eauto.
-      + intros [[x tau] f] s1. eapply pre_existential. intros C1.
-        eapply pre_existential. intros C2. eapply pre_existential. intros S'. 
-        eapply pre_uncurry_r. intros [Hvar [Hsubst [Haplha Hctx]]].
-        eapply bind_triple.
-        * eapply get_vars_project_vars_sound; [ eassumption | | | eassumption ].
-          intros x' Hx'. eapply Hbin1. now eauto.
-          eapply binding_not_in_map_antimon; [| eassumption ].
-          eapply Included_Union_compat; [| now apply Included_refl ].
-          now eapply project_var_free_set_Included; eauto.
-        * intros [xs f'] _. eapply pre_existential. intros C1'.
-          eapply pre_existential. intros C2'. eapply pre_existential. intros S''. 
-          eapply pre_uncurry_r. intros [Hvars [Hall [Halpha' Hctx']]]. eapply bind_triple.
-          eapply get_name_fresh.
-          intros x' i. eapply pre_uncurry_l. intros Hf1.
-          eapply bind_triple.
-          now eapply get_name_fresh. 
-          intros x'' s2. eapply pre_uncurry_l. intros Hf2. 
-          eapply bind_triple. eapply get_typeinfo_preserves_prop.
-          intros tinf s3. eapply return_triple.
-          intros s4 Hf3. simpl. exists (comp_ctx_f C2 C2').
-          split. intros e. rewrite <- app_ctx_f_fuse. congruence.
-          split; eauto.
-          repeat eexists. 
-          econstructor;
-            [ | econstructor; eassumption | eapply Hf1; now apply Pos.le_refl
-              | eapply Hf2; now apply Pos.le_refl
-              | intros Hc; subst x';  eapply Hf2;
-                [ now apply Pos.le_refl | now eauto ]].
-          rewrite !Union_assoc. eapply Disjoint_sym. eapply Disjoint_Union; eapply Disjoint_sym. 
-          rewrite <- Union_assoc. eapply Disjoint_free_set; [| eassumption ].
-          eapply binding_not_in_map_antimon; [| eassumption ]. now apply Included_Union_l.
-          eapply Disjoint_Included_r; [| eassumption ]. do 2 apply Included_Union_mon_r.
-          now apply Included_refl.
-          intros e e' He. rewrite <- !app_ctx_f_fuse. now eauto.
-          assert (Hinj' : injective ((subst FVmap) {x' ~> x'})).
-          { rewrite f_eq_extend_same. eassumption.
-            unfold subst. rewrite Hbin2; eauto.
-            left. eapply project_var_free_set_Included. eassumption.
-            eapply project_vars_free_set_Included. eassumption.
-            eapply Hf1. zify; omega. }
-          econstructor. eassumption. eassumption.
-          econstructor. eapply extend_same. eassumption.
-          rewrite f_eq_extend_same. eassumption.
-          eapply extend_same. unfold subst. rewrite Hbin2. reflexivity.
-          left. eapply project_var_free_set_Included. eassumption.
-          eapply project_vars_free_set_Included. eassumption.
-          eapply Hf2. zify; omega. 
-          constructor. constructor. do 2 eapply extend_same.
-          unfold subst. rewrite Hbin2. reflexivity.
-          left. eapply project_var_free_set_Included. eassumption.
-          eapply project_vars_free_set_Included. eassumption.
-          eapply Hf2. zify; omega.
-          eapply Forall2_same. intros z Hin. do 2 eapply extend_same.
-          eapply Forall_forall with (P := fun z => subst FVmap z = z).
-          eapply Forall2_Forall with (P := fun z z' => subst FVmap z = z').
-          eassumption. eassumption.
-          do 2 eapply extend_same.
-          unfold subst. rewrite Hbin2. reflexivity.
-          left. eapply project_var_free_set_Included. eassumption.
-          eapply project_vars_free_set_Included. eassumption.
-          eapply Hf1. zify. omega.
-          eapply fresh_monotonic; [| eassumption ]. 
-          do 2 eapply Setminus_Included. eapply Included_trans.
-          now eapply project_vars_free_set_Included; eauto.
-          now eapply project_var_free_set_Included; eauto.
-    - eapply pre_post_mp_r. eapply bind_triple.
-      + eapply get_vars_project_vars_sound; [ eassumption | | eassumption | eassumption ].
-        intros x Hx. eapply Hbin1. eauto.
-      + intros [xs f] s. eapply pre_eq_state.
-        intros [x'' d''] [C [C' [S' [Hf [Hproj [Hsub [Halpha Hctx]]]]]]].
-        eapply pre_post_mp_l.
-        eapply bind_triple.
-        eapply H with (Scope := Union var (Singleton var v) Scope)
-                      (S := S')
-                      (FVmap := Maps.PTree.set v (BoundVar t) FVmap).
-        * eapply FVmap_inv_set_bound. eassumption. 
-        * rewrite <- subst_BoundVar_f_eq. eapply not_In_new_function_names_injective.
-          intros Hc. eapply HD3. now eauto. assumption.
-        * eapply binding_in_map_antimon; [| eapply binding_in_map_set; eassumption ].
-          now eapply occurs_free_Eprim_Included.
-        * eapply binding_not_in_map_antimon.
-          apply Included_Union_compat. now eapply project_vars_free_set_Included; eauto.
-          now apply Included_refl.
-          eapply binding_not_in_map_set_not_In_S. eassumption.  
-          intros Hc; inv Hc. now eapply HD1; eauto. inv H0; eapply HD2; eauto.
-        * rewrite bound_var_Eprim, occurs_free_Eprim in HD1.
-          eapply Disjoint_Included_l. now eapply project_vars_free_set_Included; eauto.
-          eapply Disjoint_Included_r; [| eassumption ]. rewrite <- Union_assoc.
-          apply Included_Union_compat. now apply Included_refl.
-          rewrite Union_assoc.
-          apply Included_Union_compat; [| now apply Included_refl ].
-          rewrite Union_sym, <- Union_assoc. eapply Included_Union_mon_r.
-          rewrite <- (@Union_Setminus _ _ _ _). now apply Included_Union_l.
-        * intros Hc. inv Hc; eapply HD2; eauto.
-          rewrite bound_var_Eprim, occurs_free_Eprim.
-          destruct (Coqlib.peq Γ v); subst;  eauto.
-          right. right. constructor; eauto. intros Hc; inv Hc. congruence.
-        * eapply Disjoint_Included_l;[ now apply new_function_names_set_BoundVar | ].
-          eapply Disjoint_Included_r; [| eassumption ].
-          rewrite bound_var_Eprim, occurs_free_Eprim.
-          rewrite <- !Union_assoc. apply Included_Union_mon_r.
-          rewrite !Union_assoc, (Union_sym _ (Singleton var v)), !Union_assoc.
-          apply Included_Union_compat; [| now apply Included_refl ].
-          rewrite (@Setminus_Union_Included _ _ _ _ _).
-          now apply Included_Union_r. now apply Included_refl.
-        * intros e' s'. eapply return_triple. intros s'' Hf' Hcc. subst.
-          edestruct (Hf' Hf) as [C'' [HC'' [[e'' [Ce [Hcc [Ha1 Ha2]]]] Hf'']]]; eauto. 
-          exists C'. split. now eauto. split. do 2 eexists. split.
-          econstructor. 
-          rewrite !Union_assoc. eapply Disjoint_sym. eapply Disjoint_Union; eapply Disjoint_sym. 
-          rewrite <- Union_assoc. eapply Disjoint_free_set; [| eassumption ].
-          eapply binding_not_in_map_antimon; [| eassumption ]. now apply Included_Union_l.
-          eapply Disjoint_Included_r; [| eassumption ]. do 2 apply Included_Union_mon_r.
-          now apply Included_refl.
-          eassumption. eassumption. 
-          split. eassumption. constructor. eassumption.
-          eapply not_In_new_function_names_injective.
-          intros Hc. eapply HD3; eauto. eassumption.
-          rewrite subst_BoundVar_f_eq. rewrite HC''. now eauto.
-          eapply fresh_monotonic. now eapply project_vars_free_set_Included; eauto.
-          eassumption.
-    - eapply pre_post_mp_r. eapply bind_triple.
-      now apply get_typeinfo_preserves_prop.
-      intros tau s1. eapply bind_triple. now apply get_name_fresh.
-      intros x s2. apply pre_uncurry_l. intros Hf1. 
-      eapply pre_post_mp_l. eapply bind_triple.
-      assert (Hincl : Included var (Union var (bound_var e) (occurs_free e))
-                               (Union var (bound_var_fundefs (Fcons v t l e f5))
-                                      (occurs_free_fundefs (Fcons v t l e f5)))).
-      { rewrite bound_var_fundefs_Fcons.
-        rewrite !Union_assoc, Union_sym with (s4 := FromList l), Union_sym with (s4 := bound_var e), <- !Union_assoc.
-        apply Included_Union_compat. now apply Included_refl.
-        eapply Included_trans. eapply occurs_free_in_fun with (B := Fcons v t l e f5).
-        econstructor. now eauto. apply Included_Union_compat. now apply Included_refl. 
-        simpl. rewrite <- Union_assoc. apply Included_Union_compat. now apply Included_refl. 
-        apply Included_Union_compat; [| now apply Included_refl ].
-        now eapply name_in_fundefs_bound_var_fundefs. }
-      eapply H with (Scope := FromList l) (Funs := Funs) (FVs := FVs) (S := Setminus _ S (Singleton _ x)).
-      + rewrite <- Union_Empty_set_r with (s := FromList l). eapply FVmapInv_add_params.
-        eassumption.
-      + eapply injective_add_params; [| eassumption].
-        eapply Disjoint_Included_r; [| eassumption ]. left. eauto.
-      + eapply binding_in_map_antimon; [| eapply binding_in_map_add_params; eassumption ].
-        rewrite Union_sym. rewrite Union_sym with (s3 := occurs_free_fundefs _ ).
-        eapply occurs_free_in_fun. constructor. eauto.
-      + intros x'. rewrite <- (@Union_Setminus _ _ _ _), Union_Included_Same_set. 
-        eapply binding_not_in_map_add_params. eassumption.
-        constructor. intros y Hc. inv Hc. eapply HD1. constructor; eauto. now right; eauto.
-        intros x'' Hc; inv Hc. eapply Hf1. zify; omega.
-      + rewrite Union_assoc. eapply Disjoint_sym. eapply Disjoint_Union.
-        eapply Disjoint_Included_r. now apply Subset_Setminus.
-        eapply Disjoint_sym. eapply Disjoint_Included_r; [| eassumption ].
-        apply Included_Union_mon_r. eassumption.
-        eapply Disjoint_sym. eapply Disjoint_Setminus. now apply Included_refl.
-      + intros Hc. eapply HD1. inv Hc.
-        constructor; [ | now eauto ]; eapply Hf1; zify; omega.
-        constructor. eapply Hf1; zify; omega. right.
-        eapply occurs_free_in_fun with (B := Fcons v t l e f5) in H1; [| econstructor; now eauto ].
-        inv H1; eauto. inv H2; eauto. left. now eapply name_in_fundefs_bound_var_fundefs. 
-      + eapply Disjoint_Included_l. apply new_function_names_add_params.
-        eapply Disjoint_Included_r; [| eassumption ]. rewrite Union_sym. eassumption. 
-      + intros [e' f] s3. eapply pre_post_mp_l. eapply bind_triple.
-        eapply H0 with (S := Setminus _ S (Singleton _ x)); [ eassumption | eassumption | | | | | ].
-        * eapply binding_in_map_antimon; [| eassumption ].
-          simpl. rewrite Union_assoc. apply Included_Union_compat.
-          now apply occurs_free_fundefs_Fcons_Included. now apply Included_refl.
-        * eapply binding_not_in_map_antimon. now apply Subset_Setminus.
-          eassumption.
-        * eapply Disjoint_Included_l. now apply Subset_Setminus.
-          eapply Disjoint_Included_r; [| eassumption ].
-          apply Included_Union_compat. now apply Included_refl.
-          rewrite bound_var_fundefs_Fcons. rewrite Union_sym with (s4 := Singleton var v).
-          do 2 rewrite <- Union_assoc. rewrite Union_sym with (s4 := Singleton var v).
-          apply Included_Union_mon_r.
-          apply Included_Union_compat. now apply Included_Union_r.
-          now apply occurs_free_fundefs_Fcons_Included.
-          (* TODO make this a lemma *)
-        * eapply Disjoint_Included_r; [| eassumption ]. 
-          rewrite bound_var_fundefs_Fcons. rewrite Union_sym with (s4 := Singleton var v).
-          do 2 rewrite <- Union_assoc. rewrite Union_sym with (s4 := Singleton var v).
-          apply Included_Union_mon_r.
-          apply Included_Union_compat. now apply Included_Union_r.
-          now apply occurs_free_fundefs_Fcons_Included.
-        * eapply Included_trans; [| eassumption ]. now apply Included_Union_r.
-        * intros B' s5.
-          assert (Ha: exists v' tau1 tau2, Maps.PTree.get v FVmap = Some (MRFun v' tau1 tau2)).
-          { destruct Minv as [_ [HM _]]. eapply HM. rewrite Setminus_Empty_set_Same_set.
-            eapply Hinc. left; eauto. }
-          destruct Ha as [v' [tau1 [tau2 Ha']]]. rewrite Ha'.
-          eapply return_triple. intros s6 Hcc1 Hcc2 Hf.
-          (* add params gives the same substitution *)
-          edestruct (Hcc2 Hf) as [C1 [Hctx1 [[e'' [C1' [Hcc [Ha1 Ha2]]]] Hf1']]].
-          destruct (Hcc1 Hf1') as [[B'' [Hcc1' Ha1']] Hf2'].
-          split; [| eapply fresh_monotonic; [ now apply Subset_Setminus | eassumption ]].
-          eexists. split. constructor; [| eassumption | eassumption ]. intros Hc.
-          eapply HD1 with (x:=x). constructor. eapply Hf1. zify. omega.
-          inv Hc; eauto. inv H1; now right; eauto.
-          edestruct construct_lst_injection_add_params as [f' [Hfeq Hinj']].
-          eapply Disjoint_Included_r; [| eassumption ]. left. now eauto. eassumption.
-          rewrite <- Hfeq in Ha2. 
-          econstructor. unfold subst. now rewrite Ha'. reflexivity. 
-          eassumption. constructor. eassumption. 
-          rewrite Hfeq. rewrite f_eq_extend_same. eapply injective_add_params.
-          eapply Disjoint_Included_r; [| eassumption ]. left. now eauto. eassumption.
-          eapply binding_not_in_map_add_params in Hbin2.  
-          unfold subst. rewrite Hbin2. reflexivity. eapply Hf1. zify; omega.
-          eapply Disjoint_Included_r; [| eassumption ]. now right; eauto.
-          rewrite f_eq_extend_same, Hctx1. rewrite <- Hfeq in Ha1. now eauto.
-          rewrite Hfeq. eapply binding_not_in_map_add_params in Hbin2.  
-          unfold subst. rewrite Hbin2. reflexivity. eapply Hf1. zify; omega.
-          eapply Disjoint_Included_r; [| eassumption ]. right. now eauto.      
-    - eapply return_triple. intros Hc _ Hf.
-      split; [| eassumption ]. eexists. now split; constructor.
-    Admitted.
- *)
-  Abort.
-
-End CC_correct.
